Clean the Coq development

Galois.v
@@ -4,104 +4,372 @@ Set Implicit Arguments.
 Unset Strict Implicit.
 Unset Printing Implicit Defensive.
 
-Require Import ClassicalExtras. 
+Require Import ClassicalExtras.
+Require Import MyNotation.
+Require Import FunctionalExtensionality.
+Require Import PropExtensionality.
+Definition prop_extensionality := propositional_extensionality.
 
-Notation "π1 ⊆ π2" := (forall t, π1 t -> π2 t) (at level 50).
-
-Lemma subset_trans {X : Set} (π1 π2 π3 : X -> Prop) :
-  π1 ⊆ π2 -> π2 ⊆ π3 -> π1 ⊆ π3.
-Proof.
-  move => H1 H2 x π1_x. apply: H2. by apply: H1.  
-Qed.
-
-Lemma subset_ref {X : Set} (π : X -> Prop) :
-  π ⊆ π.
-Proof. by move => t. Qed. 
-
-Definition monotone {X Y : Set} (f : (X -> Prop) -> (Y -> Prop)) : Prop :=
+Definition monotone {X Y : Type} (f : (X -> Prop) -> (Y -> Prop)) : Prop :=
   forall (π1 π2: X -> Prop), (π1 ⊆ π2) -> (f π1 ⊆ f π2).
 
-Definition idempotent {X : Set} (f : (X -> Prop) -> (X -> Prop)) : Prop :=
+Definition idempotent {X : Type} (f : (X -> Prop) -> (X -> Prop)) : Prop :=
   forall π: X -> Prop, f (f π) = f π.
 
-Definition extensive {X : Set} (f : (X -> Prop) -> (X -> Prop)) : Prop :=
+Definition extensive {X : Type} (f : (X -> Prop) -> (X -> Prop)) : Prop :=
   forall π: X -> Prop, π ⊆ (f π).
 
-Definition Adjunction_law {A C : Set}
+
+Definition lift {X Y : Type} (f :(X -> Prop) -> (Y -> Prop))
+                            (H : (X -> Prop) -> Prop) : ((Y -> Prop) -> Prop) :=
+  fun (b1 : Y -> Prop) => exists b2, (H b2) /\ b1 = f b2.
+
+(* Definition of the adjunction law *)
+
+Definition Adjunction_law {A C : Type}
            (α : (C -> Prop) -> (A -> Prop))
-           (γ : (A -> Prop) -> (C -> Prop)) := 
-  forall (a: A -> Prop) (c: C -> Prop),  (α c) ⊆ a <-> c ⊆ (γ a). 
-    
-
-(* We define Galois connection between powersets ordered by set inclusion
-
-   (2^X, ⊆) ⇆ (2^Y, ⊆) 
-
-*)
-
-Record Galois_connection (A C : Set) := {
-
-         α : (C -> Prop) -> (A -> Prop);
-         γ : (A -> Prop) -> (C -> Prop);
-
-         ajunction_law : Adjunction_law α γ
-
-        }.
+           (γ : (A -> Prop) -> (C -> Prop)) :=
+  forall (a: A -> Prop) (c: C -> Prop),  (α c) ⊆ a <-> c ⊆ (γ a).
 
 
-Definition Galois_fst {A C : Set}
+(* We define Galois connection between powersets ordered by set inclusion:
+     (2^X, ⊆) ⇆ (2^Y, ⊆)
+   *)
+Structure Galois_Connection (A C : Type) := {
+    α : (C -> Prop) -> (A -> Prop);
+    γ : (A -> Prop) -> (C -> Prop);
+    adjunction_law : Adjunction_law α γ
+  }.
+
+
+Definition Galois_fst {A C : Type}
            (α: (C -> Prop) -> (A -> Prop))
            (γ: (A -> Prop) -> (C -> Prop)) :=
   forall (c: C -> Prop),  c ⊆ (γ (α c)).
 
-Definition Galois_snd {A C : Set} 
+Definition Galois_snd {A C : Type}
            (α: (C -> Prop) -> (A -> Prop))
            (γ: (A -> Prop) -> (C -> Prop)) :=
   forall (a : A -> Prop), (α (γ a)) ⊆ a.
 
-Lemma Galois_equiv {A C: Set}
-       (α: (C -> Prop) -> (A -> Prop))
-       (γ: (A -> Prop) -> (C -> Prop)) :
-
-  Adjunction_law α γ <-> ( monotone α /\ monotone γ /\ Galois_fst α γ  /\ Galois_snd α γ). 
+Lemma Galois_equiv {A C: Type}
+      (α: (C -> Prop) -> (A -> Prop))
+      (γ: (A -> Prop) -> (C -> Prop)) :
+  Adjunction_law α γ <-> ( monotone α /\ monotone γ /\ Galois_fst α γ  /\ Galois_snd α γ).
 Proof.
   split.
   - move => H_adj. split.
-    + move => c1 c2 H_sub. rewrite H_adj. 
+    + move => c1 c2 H_sub. rewrite H_adj.
       apply: (subset_trans H_sub). by rewrite -H_adj.
     + split.
       ++ move => a1 a2 H_sub. rewrite -H_adj.
          apply: subset_trans. rewrite H_adj. by apply: subset_ref.
          assumption.
-      ++ split; move => x; [by rewrite -H_adj | by rewrite H_adj]. 
+      ++ split; move => x; [by rewrite -H_adj | by rewrite H_adj].
   - move => [mono_α [mono_γ [G1 G2]]] a c. split => H.
     + apply: subset_trans. apply: (G1 c). by apply: mono_γ.
       apply: subset_trans. apply: mono_α. exact H. by apply: G2.
 Qed.
 
-(* Given ∼ ⊆ 2^C × 2^A there is a pair of maps 
+(* Galois Insertion (α (γ a)) = a *)
+Definition Insertion_snd {A C : Type}
+           (α: (C -> Prop) -> (A -> Prop))
+           (γ: (A -> Prop) -> (C -> Prop)) :=
+  forall (a : A -> Prop), (α (γ a)) = a.
 
-   α : 2^C -> 2^A,  γ : 2^A -> 2^C, that is a Galois connection 
+Structure Galois_Insertion (A C : Type) := {
+            α__i : (C -> Prop) -> (A -> Prop);
+            γ__i : (A -> Prop) -> (C -> Prop);
+            mono_α : monotone α__i;
+            mono_γ : monotone γ__i;
+            G1 : Galois_fst α__i γ__i;
+            I2 : Insertion_snd α__i γ__i
+          }.
 
-   between (2^C, ⊆) and (2^A, ⊆).    
 
+Lemma Insertion_coercion_Connection {A C : Type} :
+  Galois_Insertion A C -> Galois_Connection A C.
+Proof.
+  move => [α γ mono_alpha mono_gamma H1 H2].
+  have H_adj: Adjunction_law α γ.
+  rewrite Galois_equiv. repeat split; auto.
+  move => a. rewrite (H2 a). now apply: subset_ref.
+  exact (Build_Galois_Connection H_adj).
+Qed.
+
+Coercion Insertion_coercion_Connection  : Galois_Insertion >-> Galois_Connection.
+
+(* Galois Reflection (γ (α c)) = c *)
+
+Definition Reflection_fst {A C : Type}
+           (α: (C -> Prop) -> (A -> Prop))
+           (γ: (A -> Prop) -> (C -> Prop)) :=
+  forall (c : C -> Prop), (γ (α c)) = c.
+
+Structure Galois_Reflection (A C : Type) := {
+            α__r : (C -> Prop) -> (A -> Prop);
+            γ__r : (A -> Prop) -> (C -> Prop);
+            mono_α__r : monotone α__r;
+            mono_γ__r: monotone γ__r;
+            R1 : Reflection_fst α__r γ__r;
+            G2 : Galois_snd α__r γ__r
+          }.
+
+Lemma Reflection_coercion_Connection {A C : Type} :
+  Galois_Reflection A C -> Galois_Connection A C.
+Proof.
+  move => [α γ mono_alpha mono_gamma H1 H2].
+  have H_adj: Adjunction_law α γ.
+  rewrite Galois_equiv. repeat split; auto.
+  move => a. rewrite (H1 a). now apply: subset_ref.
+  exact (Build_Galois_Connection H_adj).
+Qed.
+
+Coercion Reflection_coercion_Connection  : Galois_Reflection >-> Galois_Connection.
+
+
+  (* Given ∼ ⊆ 2^C × 2^A there is a pair of maps
+     α : 2^C -> 2^A,  γ : 2^A -> 2^C, that is a Galois connection
+     between (2^C, ⊆) and (2^A, ⊆).
+   *)
+
+Definition low_rel  {A C : Type} (rel : C -> A -> Prop) : (C -> Prop) -> (A -> Prop) :=
+  fun (c : C -> Prop) =>
+    (fun (x : A) => exists (y : C), (c y) /\ rel y x).
+
+Definition up_rel {A C : Type} (rel : C -> A -> Prop) : (A -> Prop) -> (C -> Prop) :=
+  fun (a : A -> Prop) =>
+    (fun (y : C) => forall (x : A), (rel y x -> a x)).
+
+Lemma induced_adj_law {A C : Type} (rel : C -> A -> Prop) :
+  Adjunction_law (low_rel rel) (up_rel rel).
+Proof.
+  move => a c. rewrite /low_rel /up_rel. split.
+  + move => H t h_t t' rel_t_t'. apply: H. by exists t.
+                                               + move => H x [y [c_y rel_y_x]]. by apply: (H y).
+Qed.
+
+Definition induced_connection {A C : Type} (rel : C -> A -> Prop) : Galois_Connection A C :=
+  Build_Galois_Connection (induced_adj_law rel).
+
+ (*
+    We can also build a connection such that C is the abstract domain and A the concrete one
+
+  *)
+
+Definition swap_rel {A C : Set} (rel : C -> A -> Prop) : A -> C -> Prop := fun a c => rel c a.
+
+Definition induced_connection_swap {A C : Set} (rel : C -> A -> Prop) : Galois_Connection C A :=
+  Build_Galois_Connection (induced_adj_law (swap_rel rel)).
+
+
+(*
+  motivation:
+    we have in mind a scenario in which more observations are possible in the
+    target language, but no really "new" computations happen.
+    So that we relate a source trace with all the target traces that insert
+    extra observations between source events.
  *)
 
-Definition low_rel  {A C : Set} (rel : C -> A -> Prop) : (C -> Prop) -> (A -> Prop) :=
-  fun (c : C -> Prop) =>
-    (fun (x : A) => exists (y : C), (c y) /\ rel y x).  
+Definition total_fun_A_C {A C : Set} (rel : C -> A -> Prop) : Prop :=
+  forall a, exists! c, rel c a.
 
-Definition up_rel {A C : Set} (rel : C -> A -> Prop) : (A -> Prop) -> (C -> Prop) :=
-  fun (a : A -> Prop) =>
-    (fun (y : C) => forall (x : A), (rel y x -> a x)). 
+Definition total {A C : Type} (rel : C -> A -> Prop) : Prop :=
+  forall c, exists a, rel c a.
 
-Lemma induced_adj_law {A C : Set} (rel : C -> A -> Prop) :
-  Adjunction_law (low_rel rel) (up_rel rel). 
-Proof. 
-  move => a c. rewrite /low_rel /up_rel. split. 
-  + move => H t h_t t' rel_t_t'. apply: H. by exists t.
-  + move => H x [y [c_y rel_y_x]]. by apply: (H y).
+Definition more_obs_rel {A C : Set} (rel : C -> A -> Prop) :=
+  total_fun_A_C rel /\ total rel.
+
+
+Definition swap_low {A C : Set} (rel : C -> A -> Prop) : (A -> Prop) -> (C -> Prop) :=
+  low_rel (swap_rel rel).
+
+Definition swap_up {A C : Set} (rel : C -> A -> Prop) : (C -> Prop) -> (A -> Prop) :=
+  up_rel (swap_rel rel).
+
+Lemma monotone_swap_low {A C : Set} (rel : C -> A -> Prop) :
+  @monotone A C (swap_low rel).
+Proof.
+   have: Adjunction_law (swap_low rel) (swap_up rel)
+    by apply: adjunction_law (induced_connection (swap_rel rel)).
+   rewrite Galois_equiv. by move => [H1 [H2 [G1 G2]]].
+Qed.
+
+Lemma monotone_swap_up {A C : Set} (rel : C -> A -> Prop) :
+  @monotone C A (swap_up rel).
+Proof.
+   have: Adjunction_law (swap_low rel) (swap_up rel)
+    by apply: adjunction_law (induced_connection (swap_rel rel)).
+   rewrite Galois_equiv. by move => [H1 [H2 [G1 G2]]].
+Qed.
+
+Lemma G1_swap_up_low_leq {A C : Set} (rel : C -> A -> Prop):
+  Galois_fst (swap_low rel) (swap_up rel).
+Proof.
+  have: Adjunction_law (swap_low rel) (swap_up rel)
+    by apply: adjunction_law (induced_connection (swap_rel rel)).
+  rewrite Galois_equiv. by move => [H1 [H2 [G1 G2]]].
+Qed.
+
+Lemma I2_swap_low_up_id {A C : Set} (rel : C -> A -> Prop):
+  more_obs_rel rel ->
+  Insertion_snd (swap_low rel) (swap_up rel).
+Proof.
+  move => [rel_fun rel_total].
+  rewrite /Insertion_snd /swap_low /swap_up /low_rel /up_rel /swap_rel /=.
+  move => π__a. apply: functional_extensionality => c.
+  apply: prop_extensionality. split.
+  + move => [a [Ha rel_c_a]]. by apply: Ha.
+  + move => π_c. destruct (rel_total c) as [a rel_c_a].
+    exists a. split; auto.
+    move => c' rel_c'_a. destruct (rel_fun a) as [c_unique [rel_cunique Hunique]].
+    have H1: c_unique = c by apply: Hunique.
+    have H2: c_unique = c' by apply: Hunique.
+    by subst.
+Qed.
+
+Definition induced_insertion_swap {A C : Set}
+                                  (rel : C -> A -> Prop)
+                                  (H_obs_rel : more_obs_rel rel) : Galois_Insertion C A :=
+  @Build_Galois_Insertion C A (swap_low rel) (swap_up rel)
+                              (@monotone_swap_low A C rel)
+                              (@monotone_swap_up A C rel)
+                              (@G1_swap_up_low_leq A C rel)
+                              (@I2_swap_low_up_id A C rel H_obs_rel).
+
+
+(** *upper closure operator  \cite{giacobazzi2018abstract} (pag 7) *)
+Record Uco {X: Type} :=
+  {
+    uco: (X -> Prop) -> (X -> Prop);
+    mono: monotone uco;
+    idmp: idempotent uco;
+    ext : extensive uco
+  }.
+
+(* for simplicity defined only on insertions *)
+Definition best_approximation {A C : Set} (gal : Galois_Insertion C A)
+                                          (f : (C -> Prop) -> (C -> Prop)) : (A -> Prop) -> (A -> Prop) :=
+  (γ__i gal) ∘ f ∘ (α__i gal).
+
+
+Lemma composition_mono {A B C : Set} (f : (A -> Prop) -> (B -> Prop)) (g : (B -> Prop) -> (C -> Prop))
+      (mono_f : monotone f) (mono_g : monotone g) : monotone (g ∘ f).
+Proof.
+  move => π1 π2 H_sub. apply: mono_g. by apply: mono_f.
+Qed.
+
+
+Lemma best_approximation_mono {A C : Set} (ins : Galois_Insertion C A)
+                                          (ϕ : @Uco C) :
+                                          monotone (best_approximation ins (uco ϕ)).
+Proof.
+  rewrite /best_approximation.
+  apply: composition_mono.
+   apply: composition_mono.
+   exact (@mono_α C A ins). exact (@mono C ϕ).
+  exact (@mono_γ C A ins).
+Qed.
+
+Lemma best_approximation_idmp {A C : Set} (ins : Galois_Insertion C A)
+                                          (ϕ : @Uco C) :
+                                          idempotent (best_approximation ins (uco ϕ)).
+Proof.
+  rewrite /best_approximation /idempotent => π.
+    by rewrite (@I2 C A) (@idmp C ϕ).
+Qed.
+
+Lemma best_approximation_ext {A C : Set}  (ins : Galois_Insertion C A)
+                                          (ϕ : @Uco C) :
+                                          extensive (best_approximation ins (uco ϕ)).
+Proof.
+  rewrite /best_approximation /extensive => π.
+  apply: subset_trans.
+  exact: (@G1 C A). apply: (@mono_γ C A).
+  exact: (@ext C ϕ).
+Qed.
+
+
+Definition uco_sharp {A C : Set} (ϕ : @Uco C)
+                                 (ins : Galois_Insertion C A) : @Uco A :=
+
+  @Build_Uco A (@best_approximation A C ins (uco ϕ))
+               (@best_approximation_mono A C ins ϕ)
+               (@best_approximation_idmp A C ins ϕ)
+               (@best_approximation_ext A C ins ϕ).
+
+
+(************************************)
+(*  for relational properties       *)
+(************************************)
+
+Definition low_rel_prod  {A C : Set} (rel : C -> A -> Prop) : (C * C -> Prop) -> (A * A -> Prop) :=
+  fun c =>
+    fun a : A * A => exists x : C * C, c x /\ rel (fst x) (fst a) /\ rel (snd x) (snd a).
+
+Definition up_rel_prod {A C : Set} (rel : C -> A -> Prop) : (A * A -> Prop) -> (C * C -> Prop) :=
+  fun a =>
+    fun c : C * C => forall y : A * A, rel (fst c) (fst y) -> rel (snd c) (snd y) -> a y.
+
+Lemma induced_adj_law_prod {A C : Set} (rel : C -> A -> Prop) :
+  @Adjunction_law (A * A) (C * C) (low_rel_prod rel) (up_rel_prod rel).
+Proof.
+  move => a c. rewrite /low_rel_prod /up_rel_prod. split.
+  + move => H t h_t t' rel_t_t'_fst rel_t_t'_snd.
+    apply: H.
+    by exists t.
+  + move => H x [y [c_y [rel_y_x_1 rel_y_x_2]]]. by apply: (H y).
+Qed.
+
+Definition induced_connection_prod {A C : Set} (rel : C -> A -> Prop)
+  : Galois_Connection (A * A) (C * C) :=
+  Build_Galois_Connection (induced_adj_law_prod rel).
+
+
+Lemma rel_total_surjective {A C : Set} (rel : C -> A -> Prop):
+  more_obs_rel (swap_rel rel) -> (* total and surjective map from A to C *)
+  γ (induced_connection rel) = fun (a : A -> Prop) => (fun x : C => exists y : A, rel x y /\ a y).
+Proof.
+  move => [Hrel1 Hrel2].
+  rewrite /γ /= /up_rel. 
+  apply: functional_extensionality => a.
+  apply: functional_extensionality => x.
+  apply: prop_extensionality.
+  split.
+  + firstorder.
+  + move => [y [rel_x_y a_y]] y0 rel_x_y0.    
+    move : (Hrel2 y) => [x0 rel_x0_y].
+    move : (Hrel1 x) => [y_u rel_x_yu].
+    move: rel_x_yu. rewrite /unique. move => [rel_yu_x Hunique].
+    have hfoo0 : (swap_rel rel) y0 x by [].
+    move: (Hunique y0 hfoo0) => Heq0. subst.  
+    have hfoo  : (swap_rel rel) y x by [].
+    move: (Hunique y hfoo) => Heq. by subst.
+Qed.
+
+Lemma equal_pointwise {X : Set} (π1 π2 : X -> Prop) :
+  π1 = π2 -> (forall x : X, π1 x = π2 x).
+Proof. move => Heq x. by rewrite Heq. Qed. 
+
+Lemma rel_total_surjective_up_inj {A C : Set} (rel : C -> A -> Prop):
+  more_obs_rel (swap_rel rel) -> (* total and surjective map from A to C *)
+  (forall π1 π2, π1 <> π2 -> 
+   (γ (induced_connection rel) π1) <> (γ (induced_connection rel) π2)).
+Proof.
+  move => Hrel π1 π2 Hdiff. rewrite (rel_total_surjective Hrel) => Hf.
+  apply: Hdiff.
+  apply: functional_extensionality => a.
+  apply: prop_extensionality.
+  move: Hrel. rewrite /swap_rel /=. move =>  [Hrel1 Hrel2]. 
+  move: (Hrel2 a) => [c rel_a_c]. move: (Hrel1 c) => [unique_a [rel_unique_c Hunique]].
+  split => Hπi.
+  have [a' [rel_c_a' π2_a']] : exists a': A, rel c a'  /\ (π2 a').
+  { move: (equal_pointwise Hf c) => Heq. rewrite -Heq.
+    by exists a. } 
+  move: (Hunique a rel_a_c) (Hunique a' rel_c_a') => Heq1 Heq2. by subst.
+  (* symmetric case *)
+  have [a' [rel_c_a' π2_a']] : exists a': A, rel c a'  /\ (π1 a').
+  { move: (equal_pointwise Hf c) => Heq. rewrite Heq.
+    by exists a. } 
+  move: (Hunique a rel_a_c) (Hunique a' rel_c_a') => Heq1 Heq2. by subst.
 Qed. 
-
-Definition induced_connection {A C : Set} (rel : C -> A -> Prop) : Galois_connection A C :=
-  Build_Galois_connection (induced_adj_law rel).  
