ANI.v
@@ -1,0 +1,146 @@
+From mathcomp Require Import all_ssreflect.
+
+Set Implicit Arguments.
+Unset Printing Implicit Defensive.
+
+Require Import ClassicalExtras.
+Require Import MyNotation.
+Require Import Setoid.
+Require Import FunctionalExtensionality.
+Require Import Setoid.
+
+Require Import Galois.
+Require Import LanguageModel.
+Require Import TraceModel.
+Require Import Properties.
+Require Import ChainModel.
+Require Import Def.
+Require Import TraceCriterion. 
+
+Require Import PropExtensionality.
+Definition prop_extensionality := propositional_extensionality.
+
+Section ANI.
+
+  Variable Source Target: Language.
+  Variable compilation_chain : CompilationChain Source Target.
+
+  Variable trace__S trace__T : Set.
+
+  Local Definition prop__S := prop trace__S.
+  Local Definition prop__T := prop trace__T.
+
+  Variable Source_Semantics : Semantics Source trace__S.
+  Variable Target_Semantics : Semantics Target trace__T.
+
+  Local Definition sem__S := sem Source_Semantics.
+  Local Definition beh__S := beh Source_Semantics.
+  Local Definition sem__T := sem Target_Semantics.
+  Local Definition beh__T := beh Target_Semantics.
+  Local Definition prg__S := prg Source.
+  Local Definition prg__T := prg Target.
+  Local Definition sat__S := sat Source_Semantics.
+  Local Definition sat__T := sat Target_Semantics.
+  Local Definition hsat__S := hsat Source_Semantics.
+  Local Definition hsat__T := hsat Target_Semantics.
+
+  Local Definition cmp := compile_whole Source Target compilation_chain.
+
+  Local Notation "W ↓" := (cmp W) (at level 50).
+
+  Variable rel : trace__S -> trace__T -> Prop.
+  Variable H_rel : more_obs_rel rel. 
+
+  Local Definition ins : Galois_Insertion trace__S trace__T :=
+    induced_insertion_swap H_rel.
+
+  Lemma swap_low_t_single (s : trace__S) (t : trace__T) (rel_s_t : rel s t) :
+    (swap_low rel) (single t) = single s.
+  Proof.
+    apply: functional_extensionality => s'.
+    apply: prop_extensionality. rewrite /single /α__i /= /swap_low /low_rel /swap_rel.
+    split.
+    + move => [t' [Heq rel_s_t']]. subst.
+      destruct H_rel as [Hrel1 Hrel2].
+      destruct (Hrel1 t) as [ss [Hss Hunique]].
+      by rewrite -(Hunique s' rel_s_t') -(Hunique s rel_s_t).
+    + move => H. rewrite H. now exists t.
+  Qed.
+
+  Local Notation "U ♯" :=  (uco_sharp U ins) (at level 60).
+
+  Lemma ϕ_sharp_ϕ {ϕ : @Uco trace__S} {s1 s2 : trace__S} {t1 t2 : trace__T}
+                   (rel1  : rel s1 t1)
+                   (rel2  : rel s2 t2) :
+  (uco (ϕ ♯)) (single t1) = (uco (ϕ ♯)) (single t2) -> (uco ϕ) (single s1) = (uco ϕ) (single s2).
+  Proof.
+    rewrite /uco_sharp /best_approximation /= (swap_low_t_single rel1) (swap_low_t_single rel2) =>
+    sharp_eq.
+    have Hfoo: (swap_low rel) (swap_up rel (uco ϕ (single s1))) =
+               (swap_low rel) (swap_up rel (uco ϕ (single s2))) by rewrite sharp_eq.
+    move: Hfoo.
+    have Hfoo1 : α__i ins = swap_low rel by [].
+    have Hfoo2 : γ__i ins = swap_up rel by []. by rewrite -Hfoo1 -Hfoo2 !(I2 ins).
+  Qed.
+
+  Lemma ρ_ρ_sharp  {ρ : @Uco trace__S} {s1 s2 : trace__S} {t1 t2 : trace__T}
+                   (rel1  : rel s1 t1)
+                   (rel2  : rel s2 t2) :
+    (uco ρ) (single s1) = (uco ρ) (single s2) -> (uco (ρ ♯)) (single t1) = (uco (ρ ♯)) (single t2).
+  Proof.
+    move => Heq.
+    by rewrite /uco_sharp /best_approximation /=
+               (swap_low_t_single rel1) (swap_low_t_single rel2) Heq.
+  Qed.
+
+
+  Local Definition rel_TC := rel_TC compilation_chain
+                                    Source_Semantics Target_Semantics
+                                    rel.
+
+  Definition ANI {X : Set} (ϕ ρ : @Uco X) : (X -> Prop) -> Prop :=
+    fun π : X -> Prop =>
+      forall x1 x2, π x1 -> π x2 ->
+                (uco ϕ) (single x1) = (uco ϕ) (single x2) ->
+                (uco ρ) (single x1) = (uco ρ) (single x2).
+
+  Theorem compiling_ANI (W : prg__S) (ϕ ρ : @Uco trace__S):
+    rel_TC ->
+    hsat__S W (ANI ϕ ρ) ->
+    hsat__T (W ↓) (ANI (ϕ ♯) (ρ ♯)).
+  Proof.
+    move => CCtilde Hsrc t1 t2 semWcmp1 semWcmp2 H_ϕ_sharp. 
+    destruct H_rel as [Hfun Htot].
+    destruct (Hfun t1) as [s1 [Hrel1 Hunique1]]. (* *) 
+    destruct (Hfun t2) as [s2 [Hrel2 Hunique2]].
+    destruct (CCtilde W t1 semWcmp1) as [ss1 [relss1t1 Wsem1]]. 
+    destruct (CCtilde W t2 semWcmp2) as [ss2 [relss2t2 Wsem2]].
+    move: (Hunique1 ss1 relss1t1) => Heq1.
+    move: (Hunique2 ss2 relss2t2) => Heq2. subst.  
+    move: (ϕ_sharp_ϕ Hrel1 Hrel2 H_ϕ_sharp) => Hϕ.
+    move: (Hsrc ss1 ss2 Wsem1 Wsem2 Hϕ). exact (ρ_ρ_sharp Hrel1 Hrel2).
+  Qed.
+
+  (* CA: notice that ϕ_sharp_ϕ and  ρ_ρ_sharp together provide an equivalence
+         that we do not really need.
+
+       CA: I think it is possible to weaken our assumptions,
+           what I think is strictly necessary is the folllwing
+
+           let f := swap_low rel
+               g := swap_up  rel
+
+           (for an arbitrary uco in the src and π_s)
+
+            + [to show ϕ♯ is idempotent]
+                ϕ (f (g π_s)) = π_s
+                that is much weaker than asking swap_low ∘ swap_up = id,
+                and can be reprhased as a condition on ϕ like,
+                "ϕ maps elements of the same fg-level to the same property"
+
+            +   rel s t -> ϕ(s) = ϕ (f t).
+                CA: this last requirement seems to imply the condition we imposed on rel.
+
+   *)
+
+End ANI.
