HSafetyCriterion.v
@@ -1,0 +1,104 @@
+From mathcomp Require Import all_ssreflect.
+
+Set Implicit Arguments.
+Unset Printing Implicit Defensive.
+
+Require Import ClassicalExtras.
+Require Import MyNotation.
+Require Import Setoid.
+Require Import FunctionalExtensionality.
+Require Import Setoid.
+
+Require Import Galois.
+Require Import LanguageModel.
+Require Import TraceModel.
+Require Import Properties.
+Require Import ChainModel.
+Require Import HSafetyPreservation.
+Require Import SafetyCriterion.
+
+Require Import PropExtensionality.
+Definition prop_extensionality := propositional_extensionality.
+
+Section HSafeCriterion.
+  
+  Variable Source Target: Language.
+  Variable compilation_chain : CompilationChain Source Target.
+
+  Variable T_evs S_evs : Events.
+  Variable T_end S_end : Endstates.
+
+  Local Definition trace__S := @trace S_evs S_end.
+  Local Definition finpref__S := @finpref S_evs S_end.
+  Local Definition trace__T := @trace T_evs T_end.
+  Local Definition finpref__T := @finpref T_evs T_end.
+
+  Local Definition prop__S := prop trace__S.
+  Local Definition prop__T := prop trace__T.
+  Local Definition hprop__S := hprop trace__S.
+  Local Definition hprop__T := hprop trace__T.
+
+  Local Definition HSafety__S := @HSafe S_evs S_end.
+  Local Definition HSafety__T := @HSafe T_evs T_end.
+
+
+  Variable Source_Semantics : Semantics Source trace__S.
+  Variable Target_Semantics : Semantics Target trace__T.
+
+  Local Definition sem__S := sem Source_Semantics.
+  Local Definition sem__T := sem Target_Semantics.
+  Local Definition beh__S := beh Source_Semantics.
+  Local Definition beh__T := beh Target_Semantics.
+  Local Definition prg__S := prg Source.
+  Local Definition prg__T := prg Target.
+  Local Definition ctx__S := ctx Source.
+  Local Definition ctx__T := ctx Target.
+  Local Definition hsat__S := hsat Source_Semantics.
+  Local Definition hsat__T := hsat Target_Semantics.
+
+  Local Definition cmp := compile_whole Source Target compilation_chain.
+
+  Local Notation "W ↓" := (cmp W) (at level 50).
+
+  Variable rel : trace__S -> trace__T -> Prop.
+
+  Local Definition adjunction :=  induced_connection rel.
+
+  Local Definition τ' : prop__S -> prop__T := α adjunction.
+  Local Definition σ' : prop__T -> prop__S := γ adjunction.
+
+  Local Definition rel_adjunction_law : Adjunction_law τ' σ' := adjunction_law adjunction.
+
+  Lemma τ_mono : monotone τ'.
+  Proof. move/Galois_equiv: rel_adjunction_law. by move => [H1 H2]. Qed.
+
+  Definition rel_SC : Prop := rel_SC  compilation_chain
+                                   Source_Semantics Target_Semantics
+                                   rel.
+
+  Local Definition sCl_σ : hprop__T -> hprop__S := sCl_σ σ'.
+  Local Definition hsCl_τ : hprop__S -> hprop__T := hsCl_τ τ'.
+
+  Local Definition hsCl_τhP := hsCl_τhP compilation_chain
+                                       Source_Semantics Target_Semantics
+                                       τ'.
+
+
+  Local Definition sCl_σhP := sCl_σhP compilation_chain
+                                      Source_Semantics Target_Semantics
+                                      σ'.
+
+  Local Definition  hsCl_τ_SCHP_sClσHSafeP := hsCl_τ_SCHP_sClσHSafeP
+                                              compilation_chain
+                                              Source_Semantics Target_Semantics
+                                              rel_adjunction_law. 
+  
+  Theorem rel_SC_hsClτSCHP : rel_SC <-> (forall (P : prg__S) (H__S : hprop__S), SSC H__S -> hsCl_τhP P H__S).
+  Admitted. 
+
+  Theorem rel_TC_sCl_σRSCHP : rel_SC <-> (forall (W : prg__S) (H__T : hprop__T), HSafe H__T ->  sCl_σhP W H__T).
+  Proof.
+   by rewrite hsCl_τ_SCHP_sClσHSafeP rel_SC_hsClτSCHP.
+  Qed.
+
+End HSafeCriterion.
