HyperCriterion.v
@@ -1,0 +1,178 @@
+From mathcomp Require Import all_ssreflect.
+
+Set Implicit Arguments.
+Unset Printing Implicit Defensive.
+
+Require Import ClassicalExtras.
+Require Import MyNotation.
+Require Import Setoid.
+Require Import FunctionalExtensionality.
+
+
+Require Import Galois.
+Require Import LanguageModel.
+Require Import TraceModel.
+Require Import Properties.
+Require Import ChainModel.
+Require Import Def.
+Require Import HyperDef.
+Require Import TraceCriterion.
+
+Require Import PropExtensionality.
+Definition prop_extensionality := propositional_extensionality.
+
+Section HyperCriterion.
+
+  Variable Source Target: Language.
+  Variable compilation_chain : CompilationChain Source Target.
+
+  (*CA: we don't need a particular structure of traces to define preservation
+        e.g. traces = values or our defn of traces both make sense
+   *)
+  Variable trace__S trace__T : Set.
+
+  Local Definition prop__S := prop trace__S.
+  Local Definition prop__T := prop trace__T.
+  Local Definition hprop__S := hprop trace__S.
+  Local Definition hprop__T := hprop trace__T.
+
+  Variable Source_Semantics : Semantics Source trace__S.
+  Variable Target_Semantics : Semantics Target trace__T.
+
+  Local Definition sem__S := sem Source_Semantics.
+  Local Definition sem__T := sem Target_Semantics.
+  Local Definition beh__S := beh Source_Semantics.
+  Local Definition beh__T := beh Target_Semantics.
+  Local Definition prg__S := prg Source.
+  Local Definition prg__T := prg Target.
+  Local Definition sat__S := sat Source_Semantics.
+  Local Definition sat__T := sat Target_Semantics.
+  Local Definition hsat__S := hsat Source_Semantics.
+  Local Definition hsat__T := hsat Target_Semantics.
+
+  Local Definition cmp := compile_whole Source Target compilation_chain.
+
+  Local Notation "W ↓" := (cmp W) (at level 50).
+
+  Variable rel : trace__S -> trace__T -> Prop.
+
+  Local Definition adjunction :=  induced_connection rel.
+
+  Local Definition τ' : prop__S -> prop__T := α adjunction.
+  Local Definition σ' : prop__T -> prop__S := γ adjunction.
+
+  Local Definition rel_adjunction_law : Adjunction_law τ' σ' := adjunction_law adjunction.
+
+  Local Definition τP := τTP compilation_chain
+                             Source_Semantics Target_Semantics
+                             τ'.
+
+  Local Definition σP := σTP compilation_chain
+                             Source_Semantics Target_Semantics
+                             σ'.
+
+
+  Local Definition τHP := τHP compilation_chain
+                              Source_Semantics Target_Semantics
+                              τ'.
+
+  Local Definition σHP := σHP compilation_chain
+                          Source_Semantics Target_Semantics
+                          σ'.
+
+
+  Definition rel_HC :=  forall W t__T, beh__T (W ↓) t__T <-> (exists t__S, rel t__S t__T /\ beh__S W t__S).
+
+  Lemma rel_HC' : rel_HC <-> forall W, beh__T (W ↓) = τ' (beh__S W).
+    split => Hrel W.
+    apply functional_extensionality => t__T. apply: prop_extensionality.
+    rewrite (Hrel W). by firstorder.
+    rewrite (Hrel W). by firstorder.
+  Qed.
+
+  Theorem rel_HC_τHP : rel_HC <-> τHP.
+  Proof.
+    rewrite rel_HC'. split.
+    - move => H_rel W h__S. now exists (beh__S W).
+    - move => H_τHP W. specialize (H_τHP W (fun π__S => π__S = beh__S W)).
+      have Hfoo : hsat__S W (fun π__S => π__S = beh__S W) by auto.
+      destruct (H_τHP Hfoo) as [bs [Heq H]]. subst. exact H.
+  Qed.
+
+  (*CA: if τ ⇆ σ is an insertion then
+        tilde_HC =>  σHP
+        but not able to prove the vicerversa holds
+        (quite convinced it is not true)
+  *)
+
+  Lemma rel_HC_σHP : (Insertion_snd τ' σ') ->
+    rel_HC -> σHP.
+  Proof.
+    rewrite rel_HC' => HIns Hrel W H__T [b__T [bt_HT Heq]].
+    move: (Hrel W). rewrite /beh__T /beh__S Heq HIns.
+    move => Heq__T. now subst.
+  Qed.
+
+  Lemma σHP_rel_HC : (Reflection_fst τ' σ') ->
+    σHP -> rel_HC.
+  Proof.
+    rewrite rel_HC' => Hrefl Hσpres W.
+    move: (Hσpres W (fun π__T => π__T = τ' (beh__S W))).
+    rewrite /σhP => σ_pres_behW. apply: σ_pres_behW.
+    have: (HyperDef.σ__h σ' (eq^~ (τ' (beh__S W)))) = (fun π__S => π__S = (beh__S W)).
+    { rewrite /HyperDef.σ__h /lift.
+      apply: functional_extensionality => x.
+      apply: prop_extensionality.
+      split.
+      move => [b2 [H1 H2]]. subst. apply: Hrefl. 
+      move => Heq. rewrite Heq. exists (τ' (beh__S W)).
+      split; [reflexivity | by rewrite Hrefl]. } 
+    move => Heq. by rewrite Heq.  
+   Qed. 
+    
+  (****************************************************************)
+
+  (* rel_TC /\ rel_TC_fwd -> rel_HC ? *)
+
+  Local Definition rel_TC := rel_TC compilation_chain
+                                    Source_Semantics Target_Semantics
+                                    rel.
+
+  Local Definition rel_FC1 := rel_FC1 compilation_chain
+                                      Source_Semantics Target_Semantics
+                                      rel.
+
+  Local Definition rel_FC2 := rel_FC2 compilation_chain
+                                      Source_Semantics Target_Semantics
+                                      rel.
+
+  (* under the assumption rel is a total function from source to target traces
+     HC comes as consequence of TC and FC
+   *)
+  Theorem rel_total_map_TC_plus_FC1_HC :
+   (forall s, exists! t, rel s t) ->
+    rel_TC -> rel_FC1 -> rel_HC.
+  Proof.
+   setoid_rewrite rel_TC'. setoid_rewrite rel_FC1'.
+   rewrite rel_HC' => rel_map bcc fcc W.
+   apply: mutual_inclusion.
+   + by apply: bcc.
+   + rewrite rel_adjunction_law => s behWs t rel_s_t.
+     move: (fcc W s behWs). move => [t' [rel_s_t' beh_cmpW_t']].
+     have Heq: t = t'.
+     { move: (rel_map s). move => [t0 [rel_s_t0 eq_t0]].
+         by rewrite -(eq_t0 t rel_s_t) -(eq_t0 t' rel_s_t'). }
+       by rewrite Heq.
+   Qed.
+
+  Theorem TC_plus_FC2_HC :
+    rel_TC -> rel_FC2 -> rel_HC.
+  Proof.
+    setoid_rewrite rel_TC'. setoid_rewrite rel_FC2'.
+    rewrite rel_HC' => bcc fcc W.
+    apply: mutual_inclusion.
+    + exact (bcc W).
+    + rewrite rel_adjunction_law. exact (fcc W).
+  Qed.
+
+End HyperCriterion.
