LanguageModel.v
@@ -1,0 +1,279 @@
+Set Implicit Arguments.
+
+Require Import TraceModel.
+Require Import Properties.
+Require Import ClassicalExtras.
+Require Import MyNotation.
+
+Record Language := {
+
+   prg : Type; (* Whole programs *)
+   par : Type; (* Partial programs *)
+   ctx : Type; (* Contexts *)
+   plug : par -> ctx -> prg (* Linking operation *)
+
+   }.
+
+
+(* semantics of a language can be defined over an arbitrary set *)
+
+Structure Semantics (L : Language) (trace_set : Type) := {
+
+  sem : prg L -> trace_set -> Prop;
+  non_empty_sem : forall W, exists t, sem W t
+
+  }.
+
+
+(* in case we have usual traces over events we can also have W ⇝* m for m finite prefix *)
+
+Structure EventTraceSemantics (L : Language) (Ev : Events) (Es : Endstates) := {
+                                                                                 
+  ev_semantics : Semantics L (@trace Ev Es);
+  psem W (m : @finpref Ev Es) := exists t, prefix m t /\ sem ev_semantics W t 
+  
+  }.
+
+Coercion ev_semantics : EventTraceSemantics >-> Semantics.
+
+Definition input_totality {L : Language} {Ev : Events} {Es : Endstates}
+                          (is_input : (ev Ev) -> bool)
+                          (event_semantics : EventTraceSemantics L Ev Es) : Prop :=
+  forall (W : prg L) (l : list (ev Ev)) (i1 i2: (ev Ev)),
+      (is_input i1 = true) ->
+      (is_input i1 = true) ->
+      psem event_semantics W (ftbd (snoc l i1 )) ->
+      psem event_semantics W (ftbd (snoc l i2 )).  
+
+Definition determinacy {L : Language} {Ev : Events} {Es : Endstates}
+                       (is_input : (ev Ev) -> bool)
+                       (event_semantics : EventTraceSemantics L Ev Es) : Prop :=
+  forall (W : prg L) (t1 t2 : @trace Ev Es),
+    sem (ev_semantics event_semantics) W t1 ->
+    sem (ev_semantics event_semantics) W t2 ->
+    t1 = t2 \/ (exists l i1 i2, i1 <> i2 /\ prefix (ftbd (snoc l i1)) t1 /\ prefix (ftbd (snoc l i2)) t2).  
+    
+
+Definition beh {L : Language}
+               {trace_set : Type}
+               (S : Semantics L trace_set)
+               (W : prg L) : prop trace_set :=
+  fun t => sem S W t.
+
+Definition sat {L : Language}
+               {trace_set : Type}
+               (S : Semantics L trace_set)
+               (W : prg L) (π : prop trace_set) : Prop :=
+  forall t, sem S W t -> π t.
+
+Lemma sat_upper_closed  {L : Language}
+                        {trace_set : Type}
+                        (S : Semantics L trace_set)
+                        (W : prg L ) (π1 π2 : prop trace_set) :
+  sat S W π1 -> π1 ⊆ π2 -> sat S W π2.
+Proof.
+  intros Hsat1 Hsuper t Hsem.
+  apply Hsuper.
+  now apply (Hsat1 t).
+Qed.
+
+
+Definition hsat{L : Language}
+               {trace_set : Type}
+               (S : Semantics L trace_set)
+               (W : prg L) (H : hprop trace_set) : Prop :=
+  H (beh S W).
+
+Lemma hsat_upper_closed  {L : Language}
+                         {trace_set : Type}
+                         (S : Semantics L trace_set)
+                         (W : prg L ) (H1 H2 : hprop trace_set) :
+  hsat S W H1 -> H1 ⊆ H2 -> hsat S W H2.
+Proof.
+  intros Hsat1 Hsuper.
+  apply Hsuper.
+  now apply Hsat1.
+Qed.
+
+
+Definition rsat {L : Language}
+                {trace_set : Type}
+                (S : Semantics L trace_set)
+                (P : par L) (π : prop trace_set) : Prop :=
+  forall C, sat S (plug L P C) π.
+
+Lemma rsat_upper_closed {L : Language}
+                        {trace_set : Type}
+                        (S : Semantics L trace_set)
+                        (P : par L ) (π1 π2 : prop trace_set) :
+  rsat S P π1 -> π1 ⊆ π2 -> rsat S P π2.
+Proof.
+  intros Hsat1 Hsuper C t Hsem.
+  apply Hsuper.
+  now apply (Hsat1 C t).
+Qed.
+
+Definition rhsat  {L : Language}
+                  {trace_set : Type}
+                  (S : Semantics L trace_set)
+                  (P : par L) (H : hprop trace_set) : Prop :=
+  forall C, hsat S (plug L P C) H.
+
+Lemma neg_sat  {L : Language}
+               {trace_set : Type}
+               {S : Semantics L trace_set} :
+  forall (W : prg L) (π : prop trace_set),
+    ~ sat S W π <-> exists t, sem S W t /\ ~ π t.
+Proof.
+  intros W π. unfold sat.
+  rewrite not_forall_ex_not.
+  split; intros [t H]; exists t; [now rewrite not_imp in H
+                            | now rewrite not_imp].
+Qed.
+
+(* Considering moving these two lemmas to a separate module *)
+Lemma neg_rsat {L : Language}
+               {trace_set : Type}
+               (S : Semantics L trace_set) :
+  forall (P : par L) (π : prop trace_set),
+    (~ rsat S P π <->
+     (exists C t, sem S (plug L P C) t /\ ~ π t)).
+Proof.
+  intros P π.
+  split; unfold rsat; intros H.
+  - rewrite not_forall_ex_not in H.
+    destruct H as [C H]; exists C.
+    unfold sat in H; rewrite not_forall_ex_not in H.
+    destruct H as [t H]; exists t.
+    now rewrite not_imp in H.
+  - firstorder.
+Qed.
+
+Lemma neg_rhsat {L : Language}
+                {trace_set : Type}
+                (S : Semantics L trace_set) :
+  forall P H,  (~ rhsat S P H <-> ( exists (C : ctx L), ~ H (beh S ( plug L P C )))).
+Proof.
+  intros P H.
+  split; unfold rhsat; intro H0;
+    [now rewrite <- not_forall_ex_not | now rewrite not_forall_ex_not].
+Qed.
+
+
+Lemma rhsat_upper_closed {L : Language}
+                         {trace_set : Type}
+                         (S : Semantics L trace_set)
+                         (P : par L ) (H1 H2 : hprop trace_set) :
+  rhsat S P H1 -> H1 ⊆ H2 -> rhsat S P H2.
+Proof.
+  intros rsat1 Hsuper C.
+  apply Hsuper.
+  now apply (rsat1 C).
+Qed.
+
+
+Definition sat2 {L : Language}
+                {trace_set : Type}
+                (S : Semantics L trace_set)
+                (W1 W2 : prg L) (R : trace_set * trace_set -> Prop) : Prop :=
+  forall t1 t2, sem S W1 t1 -> sem S W2 t2 -> R (t1, t2).
+
+Definition rsat2 {L : Language}
+                 {trace_set : Type}
+                 (S : Semantics L trace_set)
+                 (P1 P2 : par L) (R : trace_set * trace_set -> Prop) : Prop :=
+  forall C t1 t2, sem S (plug L P1 C) t1 -> sem S (plug L P2 C) t2 -> R (t1, t2).
+
+Lemma sat2_upper_closed  {L : Language}
+                         {trace_set : Type}
+                         (S : Semantics L trace_set)
+                         (W1 W2 : prg L ) (R1 R2 : trace_set * trace_set -> Prop) :
+  sat2 S W1 W2 R1 -> R1 ⊆ R2 -> sat2 S W1 W2 R2.
+Proof.
+  intros Hsat1 Hsuper t1 t2 Hsem1 Hsem2.
+  apply Hsuper.
+  now apply (Hsat1 t1).
+Qed.
+
+Lemma rsat2_upper_closed {L : Language}
+                         {trace_set : Type}
+                         (S : Semantics L trace_set)
+                         (P1 P2 : par L ) (R1 R2 : trace_set * trace_set -> Prop) :
+  rsat2 S P1 P2 R1 -> R1 ⊆ R2 -> rsat2 S P1 P2 R2.
+Proof.
+  intros Hsat1 Hsuper C t1 t2 Hsem1 Hsem2.
+  apply Hsuper.
+  now apply (Hsat1 C t1).
+Qed.
+
+Lemma neg_sat2  {L : Language}
+                {trace_set : Type}
+                {S : Semantics L trace_set} :
+  forall (W1 W2 : prg L) (R : trace_set * trace_set -> Prop),
+    ~ sat2 S W1 W2 R <-> exists t1 t2, sem S W1 t1 /\ sem S W2 t2 /\ ~ R (t1, t2).
+Proof.
+  intros W1 W2 R. unfold sat2.
+  rewrite not_forall_ex_not.
+  split.
+  + intros [t1 H]. rewrite not_forall_ex_not in H.
+    destruct H as [t2 H]. rewrite not_imp in H. destruct H as [H1 H].
+    rewrite not_imp in H. destruct H as [H2 H].
+    now exists t1, t2.
+  + intros [t1 [t2 [H1 [H2 H]]]].
+    exists t1. rewrite not_forall_ex_not. exists t2. firstorder.
+Qed.
+
+Lemma neg_rsat2 {L : Language}
+                {trace_set : Type}
+                (S : Semantics L trace_set) :
+  forall (P1 P2 : par L) (R: trace_set * trace_set -> Prop),
+    (~ rsat2 S P1 P2 R <->
+     (exists C t1 t2, sem S (plug L P1 C) t1 /\ sem S (plug L P2 C) t2 /\ ~ R (t1,t2))).
+Proof.
+  intros P1 P2 R.
+  split; unfold rsat2; intros H.
+  - rewrite not_forall_ex_not in H.
+    destruct H as [C H]; exists C.
+    unfold sat2 in H; rewrite not_forall_ex_not in H.
+    destruct H as [t1 H]; exists t1.
+    rewrite not_forall_ex_not in H.
+    destruct H as [t2 H]; exists t2.
+    now rewrite !not_imp in H.
+  - firstorder.
+Qed.
+
+Definition hsat2 {L : Language}
+                 {trace_set : Type}
+                 (S : Semantics L trace_set)
+                 (W1 W2 : prg L) (R : (prop trace_set) * (prop trace_set) -> Prop) : Prop :=
+  R ((beh S W1), (beh S W2)).
+
+Definition rhsat2 {L : Language}
+                  {trace_set : Type}
+                  (S : Semantics L trace_set)
+                  (P1 P2 : par L) (R : (prop trace_set) * (prop trace_set) -> Prop) : Prop :=
+  forall C, hsat2 S (plug L P1 C) (plug L P2 C) R.
+
+
+Lemma neg_rhsat2 {L : Language}
+                 {trace_set : Type}
+                 (S : Semantics L trace_set) :
+  forall P1 P2 R,  (~ rhsat2 S P1 P2 R <-> ( exists (C : ctx L),
+                                        ~ R ((beh S (plug L P1 C )),(beh S (plug L P2 C))))).
+Proof.
+  intros P1 P2 R.
+  split; unfold rhsat2; intro H0;
+    [now rewrite <- not_forall_ex_not | now rewrite not_forall_ex_not].
+Qed.
+
+
+Lemma rhsat2_upper_closed {L : Language}
+                          {trace_set : Type}
+                          (S : Semantics L trace_set)
+                          (P1 P2 : par L ) (R1 R2 : (prop trace_set) * (prop trace_set) -> Prop) :
+  rhsat2 S P1 P2 R1 -> R1 ⊆ R2 -> rhsat2 S P1 P2 R2.
+Proof.
+  intros rsat_one Hsuper C.
+  apply Hsuper.
+  now apply (rsat_one C).
+Qed.
