MyNotation.v
@@ -1,0 +1,40 @@
+From mathcomp Require Import all_ssreflect.
+
+Set Implicit Arguments.
+Unset Strict Implicit.
+Unset Printing Implicit Defensive.
+
+
+Require Import FunctionalExtensionality.
+Require Import PropExtensionality.
+Definition prop_extensionality := propositional_extensionality.
+
+(* Some preliminary lemmas and definition on subset inclusion *)
+Notation "π1 ⊆ π2" := (forall t, π1 t -> π2 t) (at level 50).
+
+Lemma subset_trans {X : Type} (π1 π2 π3 : X -> Prop) :
+  π1 ⊆ π2 -> π2 ⊆ π3 -> π1 ⊆ π3.
+Proof.
+  move => H1 H2 x π1_x. apply: H2. by apply: H1.
+Qed.
+
+Lemma subset_ref {X : Type} (π : X -> Prop) :
+  π ⊆ π.
+Proof. by move => t. Qed.
+
+Lemma mutual_inclusion {X : Type} (π1 π2 : X -> Prop) :
+  π1 ⊆ π2 -> π2 ⊆ π1 -> π1 = π2.
+Proof.
+  move => H1 H2.
+  apply: functional_extensionality => x.
+  apply: prop_extensionality. split; [by apply: H1 | by apply: H2].
+Qed.
+
+Notation "f ∘ g" := (fun x => f ( g x )) (at level 50).
+
+Definition single {X : Type} (t : X) : X -> Prop := fun x => x = t.
+
+Definition prod_map {X Y : Type} (f : (X -> Prop) -> (Y -> Prop)) : ((X -> Prop) * (X -> Prop)) ->
+                                                              ((Y -> Prop) * (Y -> Prop)) :=
+  fun x =>
+    (f (fst x), f (snd x)).
