Properties.v
@@ -1,0 +1,369 @@
+From mathcomp Require Import all_ssreflect.
+
+Set Implicit Arguments.
+Unset Strict Implicit.
+Unset Printing Implicit Defensive.
+
+Require Import FunctionalExtensionality.
+Require Import ClassicalExtras.
+Require Import MyNotation.
+
+Require Import TraceModel.
+Require Import Galois.
+
+Require Import PropExtensionality.
+Definition prop_extensionality := propositional_extensionality.
+
+(* CA: let us keep prop as more general as possible, in case
+         one day we want traces to be just values.
+ *)
+Parameter E : Events.
+Parameter Es : Endstates.
+
+Definition prop (trace_set : Type)  := trace_set -> Prop.
+Definition hprop (trace_set : Type) := (prop trace_set) -> Prop.
+Definition h_true (trace_set : Type) : hprop (trace_set) := fun (b : prop (trace_set)) => True.
+Definition hh_true (trace_set : Type) : (@hprop trace_set) -> Prop :=  fun _ => True.
+
+
+Definition fprop {E : Events} {Es: Endstates} :=
+  @finpref E Es -> Prop.
+
+Notation "M <<< b" := (forall m, M m -> exists t, b t /\ prefix m t) (at level 50).
+
+Definition Safety {E : Events}
+           {Es : Endstates}
+           (π : prop (@trace E Es)) : Prop :=
+  forall t, ~ π t ->
+       (exists m, prefix m t /\
+             (forall t', prefix m t' -> ~ π t')).
+
+(* Alternate characterization of safety *)
+Definition Safety'{E : Events}
+           {Es : Endstates}
+           (π : prop (@trace E Es)) : Prop:=
+  exists π': fprop,
+  forall t:trace, ~(π t) <-> (exists m, prefix m t /\ π' m).
+
+Lemma safety_safety'  {E : Events} {Es : Endstates} :
+  forall π, @Safety E Es π <-> @Safety' E Es π.
+Proof.
+  unfold Safety, Safety'. intro π. split; intro H.
+  - exists (fun m => forall t, prefix m t -> ~π t).
+    intros t. split; intro H'.
+    + specialize (H t H'). destruct H as [m [H1 H2]].
+      exists m. split. assumption. intros t' H. apply H2. assumption.
+    + destruct H' as [m [H1 H2]]. apply H2. assumption.
+  - intros t H0. destruct H as [π' H].
+    apply H in H0. destruct H0 as [m [H1 H2]].
+    exists m. split; try now auto.
+    intros. rewrite H. now exists m.
+Qed.
+
+Inductive Observations  {E : Events} {Es : Endstates} : (@finpref E Es -> Prop) -> Prop :=
+  empty :  Observations (fun m : finpref => False)
+| finite_union : forall M m, Observations M -> Observations (fun x => M x \/ x = m).
+
+(*****************************************************************************)
+(** *Safety closure operator                                                 *)
+(*****************************************************************************)
+
+Definition Cl  {E : Events} {Es : Endstates}
+               (π : prop (@trace E Es)) : prop (@trace E Es) :=
+  fun t => forall S, Safety S -> π ⊆ S -> S t.
+
+Lemma Cl_bigger  {E : Events} {Es : Endstates}
+                 (π: prop (@trace E Es)) : π ⊆ (Cl π).
+Proof. firstorder. Qed.
+
+Lemma Cl_Safety {E : Events} {Es : Endstates}
+                (π: prop (@trace E Es)): Safety (Cl π).
+Proof.
+  move => t not_π_t.
+  move/not_forall_ex_not: not_π_t. move => [π' H].
+  move/not_imp: H. move => [safety_π' H].
+  move/not_imp: H. move => [π_leq_π' not_π'_t].
+  destruct (safety_π' t not_π'_t) as [m [m_leq_t m_wit]].
+  exists m. split; auto. move => t' m_leq_t' Hf.
+  apply: (m_wit t'). assumption. by apply: Hf.
+Qed.
+
+Lemma Cl_id_on_Safe {E : Events} {Es : Endstates}
+                    (π: prop (@trace E Es)) :
+  Safety π -> Cl π = π.
+Proof.
+  move => Safety_π. apply: functional_extensionality => t.
+  apply: prop_extensionality.
+    by firstorder.
+Qed.
+
+Lemma Cl_smallest {E : Events} {Es : Endstates}
+                  (π: prop (@trace E Es)) :
+    forall S, Safety S -> π ⊆ S -> Cl π ⊆ S.
+Proof. by firstorder. Qed.
+
+Lemma Cl_mono {E : Events} {Es : Endstates} : monotone (@Cl E Es).
+Proof.
+  move => π1 π2 sub t cl2_t.
+  apply: cl2_t.
+  apply: Cl_Safety. apply: subset_trans. exact: sub. exact: Cl_bigger.
+Qed.
+
+Lemma Cl_idmp {E : Events} {Es : Endstates} : idempotent (@Cl E Es).
+Proof. move => π. apply: Cl_id_on_Safe. apply: Cl_Safety. Qed.
+
+
+Definition safety_uco {E : Events} {Es : Endstates} := Build_Uco (@Cl_mono E Es)
+                                                                (@Cl_idmp E Es)
+                                                                (@Cl_bigger E Es).
+
+
+Lemma Safety_Cl_prop {E : Events} {Es : Endstates} :
+  @Safety E Es = (lift (uco safety_uco)) (@h_true (@trace E Es)).
+Proof.
+  apply: functional_extensionality => π.
+  apply: prop_extensionality. split => H.
+  + exists π. split; rewrite //=.
+      by rewrite Cl_id_on_Safe.
+  + move: H. rewrite //=. move => [b [H Heq]]. subst.
+    apply: Cl_Safety.
+Qed.
+
+
+(*****************************************************************************)
+
+
+(*****************************************************************************)
+(** *Dense closure operator *)
+(*****************************************************************************)
+
+Definition Dense {E : Events} {Es : Endstates}
+                 (π: prop (@trace E Es)) : Prop :=
+  forall t, finite t -> π t.
+
+Definition dCl {E : Events} {Es : Endstates} : prop (@trace E Es) -> prop (@trace E Es) :=
+  fun π => (fun t => finite t \/ π t).
+
+Lemma Dense_dCl {E : Events} {Es : Endstates}
+                  (π: prop (@trace E Es)) : Dense (dCl π).
+Proof. firstorder. Qed.
+
+Lemma dCl_mono {E : Events} {Es : Endstates} :
+  monotone (@dCl E Es).
+Proof.
+  move => π1 π2 sub t1. rewrite /dCl.
+  move => [K1 | K2]; [by left | right; by apply: sub].
+Qed.
+
+Lemma dCl_idmp {E : Events} {Es : Endstates} :
+  idempotent (@dCl E Es).
+Proof.
+  rewrite /dCl => π.
+  apply: functional_extensionality => t.
+  apply: prop_extensionality.
+  firstorder.
+Qed.
+
+Lemma dCl_ext {E : Events} {Es : Endstates} :
+  extensive (@dCl E Es).
+Proof.
+  rewrite /dCl => π t π_t. by right.
+Qed.
+
+Lemma dCl_id_on_Dense {E : Events} {Es : Endstates}
+                      (π: prop (@trace E Es)):
+  Dense π -> dCl π = π.
+Proof.
+  rewrite /Dense /dCl => H_dense.
+  apply: functional_extensionality => t.
+  apply: prop_extensionality.
+  split; auto. move => [k | k]; [by apply: H_dense | by []].
+Qed.
+
+Definition dense_uco {E : Events} {Es : Endstates} :=
+  Build_Uco (@dCl_mono E Es)
+            dCl_idmp
+            dCl_ext.
+
+Lemma Dense_Cl_prop {E : Events} {Es : Endstates} :
+  Dense = (lift (uco dense_uco)) (@h_true (@trace E Es)).
+Proof.
+  apply: functional_extensionality => π.
+  apply: prop_extensionality.
+  split; rewrite /h_true //= => H.
+  + exists π. split; auto. by rewrite dCl_id_on_Dense.
+  + destruct H as [b [Heq H]]. subst.
+      by apply: Dense_dCl.
+Qed.
+
+(*****************************************************************************)
+
+(*CA: also for SSC hprop we only need a set of traces, not our particular model *)
+Definition SSC {trace_set : Type} (H: hprop trace_set)  : Prop :=
+  forall h, H h ->
+       (forall b : (prop trace_set), b ⊆ h -> H b).
+
+(*****************************************************************************)
+(** *SSC closure operator*)
+(*****************************************************************************)
+
+Definition sCl {trace_set : Type}
+               (H : hprop trace_set) :
+               hprop trace_set :=
+  fun b => exists b', H b' /\ b ⊆ b'.
+
+Lemma sCl_bigger {trace_set : Type} (H : hprop trace_set) : H ⊆ (sCl H).
+Proof. firstorder. Qed.
+
+Lemma sCl_SCH {trace_set : Type} (H : hprop trace_set) : SSC (sCl H).
+Proof.
+  move => h [b' [Hb' bb']] b b_h. exists b'; auto.
+Qed.
+
+Lemma sCl_id_on_SSC {trace_set : Type} (H: hprop trace_set): SSC H -> sCl H = H.
+Proof.
+  move => H_SSC. apply: functional_extensionality => b.
+  apply: prop_extensionality. firstorder.
+Qed.
+
+Lemma sCl_smallest {trace_set : Type} (H: hprop trace_set):
+  forall H', SSC H' -> H ⊆ H' -> (sCl H) ⊆ H'.
+Proof.
+  move => H' ssc_H' H_leq_H' b [b' [ b_leq_b' H_b']].
+  apply: (ssc_H' b'); auto.
+Qed.
+
+Lemma sCl_mono {trace_set : Type} (H1 H2 : hprop trace_set) :
+  H1 ⊆ H2 -> (sCl H1) ⊆ (sCl H2).
+Proof. by firstorder. Qed.
+
+Lemma sCl_idmp {trace_set : Type} (H : hprop trace_set) :
+  sCl (sCl H) = sCl H.
+Proof. apply: sCl_id_on_SSC. apply: sCl_SCH. Qed.
+
+Definition ssch_uco {trace_set : Type} : @Uco (trace_set -> Prop) :=
+  @Build_Uco (prop trace_set)
+             sCl
+             sCl_mono
+             sCl_idmp
+             sCl_bigger.
+
+
+(*****************************************************************************)
+
+(*CA: for hypersafety we need the set of traces to have structure like in our def of trace *)
+
+Definition HSafe {E : Events} {Es : Endstates}
+                 (H: hprop (@trace E Es)) :=
+  forall b, ~ H b -> (exists M, Observations M /\ M <<< b /\
+                     (forall b', M <<< b' -> ~ H b')).
+
+
+(*****************************************************************************)
+(** *HSafe closure operator*)
+(*****************************************************************************)
+
+Definition hsCl {E : Events} {Es : Endstates}
+                 (H: hprop (@trace E Es)) : (hprop (@trace E Es)) :=
+  fun b => forall Hs, HSafe Hs -> H ⊆ Hs -> Hs b.
+
+Lemma hsCl_bigger {E : Events} {Es : Endstates}
+                  (H: hprop (@trace E Es)) :  H ⊆ hsCl H.
+Proof. by firstorder. Qed.
+
+Lemma hsCl_HSafe {E : Events} {Es : Endstates}
+                 (H: hprop (@trace E Es)) : HSafe (hsCl H).
+Proof.
+  move => b. move/not_forall_ex_not => not_H_b.
+  destruct not_H_b as [H' not_H'_b].
+  move/not_imp: not_H'_b. move => [HSafe_H' not_H'_b].
+  move/not_imp: not_H'_b. move => [H_leq_H' not_H'_b].
+  destruct (HSafe_H' b not_H'_b) as [M [obs_M [M_leq_b M_wit]]].
+  exists M. repeat (split; auto).
+  move => b' M_leq_b' Hf. apply: (M_wit b'); auto.
+    by apply: Hf.
+Qed.
+
+Lemma HSafe_SCH {E : Events} {Es : Endstates} :
+  forall H, @HSafe E Es H -> SSC H.
+Proof.
+  move => H HSafe_H b Hb b' b'_leq_b.
+  apply: NNPP => not_H_b'.
+  destruct (HSafe_H b' not_H_b') as [M [obs_M [M_leq_b' M_wit]]].
+  apply: (M_wit b); firstorder.
+Qed.
+
+Lemma hsCl_id_on_HSafe {E : Events} {Es : Endstates} :
+  forall H, @HSafe E Es H -> hsCl H = H.
+Proof.
+  move => H HSafe_H.
+  apply: functional_extensionality => b.
+  apply: prop_extensionality. by firstorder.
+Qed.
+
+Lemma sCl_id_on_HSafe {E : Events} {Es : Endstates} :
+  forall H, @HSafe E Es H -> sCl H = H.
+Proof.
+  move => H HSafe_H.
+  have SSC_H: (SSC H) by apply: HSafe_SCH.
+    by rewrite (sCl_id_on_SSC SSC_H).
+Qed.
+
+Lemma hsCl_sCl {E : Events} {Es : Endstates} :
+  forall H : (hprop (@trace E Es)), sCl H ⊆ hsCl H.
+Proof.
+  move => H.
+  have ssc: SSC (hsCl H).
+  { apply: HSafe_SCH. apply: hsCl_HSafe. }
+  apply: sCl_smallest; auto.
+    by apply: hsCl_bigger.
+Qed.
+
+Lemma hsCl_smallest {E : Events} {Es : Endstates}
+                    (H: hprop (@trace E Es)):
+  forall H', HSafe H' -> H ⊆ H' -> (hsCl H) ⊆ H'.
+Proof. by firstorder. Qed.
+
+Lemma hsCl_mono {E : Events} {Es : Endstates}:
+  forall H1 H2 : hprop (@trace E Es),
+    H1 ⊆ H2 -> (hsCl H1) ⊆ (hsCl H2).
+Proof. by firstorder. Qed.
+
+Lemma hsCl_idmp  {E : Events} {Es : Endstates}
+                 (H : hprop (@trace E Es)):
+  hsCl (hsCl H) = hsCl H.
+Proof.
+  rewrite hsCl_id_on_HSafe.
+  reflexivity.
+  exact: hsCl_HSafe.
+Qed.
+
+Definition hsafe_uco {E : Events} {Es : Endstates} :
+  @Uco ((@trace E Es) -> Prop) :=
+  @Build_Uco (prop (@trace E Es))
+             hsCl
+             hsCl_mono
+             hsCl_idmp
+             hsCl_bigger.
+
+(*****************************************************************************)
+(** *2relSCH*)
+(*****************************************************************************)
+
+Definition SCH2 {trace_set : Type} (Π : (prop trace_set) * (prop trace_set) -> Prop) : Prop :=
+  forall β1 β2 β1' β2': prop trace_set,
+    Π (β1, β2) -> β1' ⊆ β1 -> β2' ⊆ β2 -> Π (β1', β2').
+
+Definition sCl2 {trace_set : Type}
+                (Π : (prop trace_set) * (prop trace_set) -> Prop) :
+                (prop  trace_set) * (prop trace_set) -> Prop  :=
+  fun b => exists b1 b2, Π (b1, b2) /\ (fst b) ⊆ b1 /\ (snd b) ⊆ b2.
+
+
+Lemma sCl2_SCH2 {trace_set : Type} (Π : (prop trace_set) * (prop trace_set) -> Prop) :
+  SCH2 (sCl2 Π).
+Proof.
+  move => β1 β2 β1' β2' [γ1 [γ2 [H_Π [Hsub1' Hbsu2']]]] H_sub1 H_sub2.
+  exists γ1, γ2. split; apply: subset_trans; eauto.
+  split; apply: subset_trans; eauto.
+Qed.
