Relation4Correctness.v
@@ -1,0 +1,88 @@
+From mathcomp Require Import all_ssreflect.
+
+Set Implicit Arguments.
+Unset Printing Implicit Defensive.
+
+Require Import ClassicalExtras.
+Require Import MyNotation.
+Require Import Setoid.
+Require Import FunctionalExtensionality.
+Require Import Setoid.
+
+Require Import Galois.
+Require Import LanguageModel.
+Require Import TraceModel.
+Require Import Properties.
+Require Import ChainModel.
+Require Import Def.
+Require Import TraceCriterion.
+
+Require Import PropExtensionality.
+Definition prop_extensionality := propositional_extensionality.
+
+Section Relation.
+
+  Variable Source Target: Language.
+  Variable compilation_chain : CompilationChain Source Target.
+
+  Variable trace__S trace__T : Set.
+
+  Local Definition prop__S := prop trace__S.
+  Local Definition prop__T := prop trace__T.
+
+  Variable Source_Semantics : Semantics Source trace__S.
+  Variable Target_Semantics : Semantics Target trace__T.
+
+  Local Definition sem__S := sem Source_Semantics.
+  Local Definition beh__S := beh Source_Semantics.
+  Local Definition sem__T := sem Target_Semantics.
+  Local Definition beh__T := beh Target_Semantics.
+  Local Definition prg__S := prg Source.
+  Local Definition prg__T := prg Target.
+  Local Definition sat__S := sat Source_Semantics.
+  Local Definition sat__T := sat Target_Semantics.
+
+  Local Definition cmp := compile_whole Source Target compilation_chain.
+
+  Local Notation "W ↓" := (cmp W) (at level 50).
+
+  (* Cheating relation *)
+  Definition rel : trace__S -> trace__T -> Prop :=
+    fun t__S t__T => exists W, sem__S W t__S /\ sem__T (W ↓) t__T.
+
+  Local Definition adjunction := induced_connection rel.
+
+  Local Definition τ' : prop__S -> prop__T := α adjunction.
+  Local Definition σ' : prop__T -> prop__S := γ adjunction.
+
+  Local Definition τTP := τTP compilation_chain
+                              Source_Semantics Target_Semantics
+                              τ'.
+
+
+  Local Definition σTP := σTP compilation_chain
+                              Source_Semantics Target_Semantics
+                              σ'.
+
+
+  Local Definition rel_TC := rel_TC compilation_chain
+                                    Source_Semantics Target_Semantics
+                                    rel.
+
+
+
+  Theorem cmp_is_rel_TC : rel_TC.
+  Proof.
+    move => W t__T W_t.
+    destruct (non_empty_sem Source_Semantics W) as [s W_s].
+    exists s. split; auto. now exists W.
+  Qed.
+
+  Corollary cmp_is_τTP: τTP.
+  Proof. setoid_rewrite <- rel_TC_τTP. exact cmp_is_rel_TC. Qed.
+
+  Corollary cmp_is_σTP : σTP.
+  Proof. setoid_rewrite <- rel_TC_σTP. exact cmp_is_rel_TC. Qed.
+
+
+End Relation.
