ResourceExhaustion.v
@@ -1,0 +1,371 @@
+Require Import ClassicalExtras.
+
+Require Import TraceModel.
+Require Import Stream.
+Require Import Properties.
+Require Import Galois.
+
+Require Import FunctionalExtensionality.
+
+Set Bullet Behavior "Strict Subproofs".
+
+
+Section ResourceExhaustion.
+  Variable event : Events.
+
+  Variable endstate : Endstates.
+
+  Definition endstateS : Endstates := endstate.
+
+  Definition out_of_memory := unit.
+  Definition endstateT : Endstates :=
+    {| es := (es endstate + out_of_memory);
+       an_es := inr tt
+    |}.
+  Definition OOM : es endstateT := inr tt.
+  Hint Unfold OOM.
+
+  Definition traceS := @trace event endstateS.
+  Definition traceT := @trace event endstateT.
+  Definition finprefS := @finpref event endstateS.
+  Definition finprefT := @finpref event endstateT.
+
+  Definition propS := @prop traceS.
+  Definition propT := @prop traceT.
+  Definition fpropS := @fprop event endstateS.
+  Definition fpropT := @fprop event endstateT.
+
+  Inductive syntactic_eq : traceS -> traceT -> Prop :=
+  | syntactic_eq_tstop : forall l e,
+      syntactic_eq (tstop l e) (tstop l ((inl e) : es endstateT))
+  | syntactic_eq_tsilent : forall l,
+      syntactic_eq (tsilent l) (tsilent l)
+  | syntactic_eq_tstream : forall s,
+      syntactic_eq (tstream s) (tstream s)
+  .
+  Notation "t__s '≡' t__t" := (syntactic_eq t__s t__t) (no associativity, at level 10).
+  Hint Constructors syntactic_eq.
+
+  Definition prefixTS (m__t : finprefT) (t__s : traceS) : Prop :=
+    match m__t with
+    | fstop l__t (inl e__t) =>
+      match t__s with
+      | tstop l__s e__s => e__t = e__s /\ l__t = l__s
+      | _ => False
+      end
+    | fstop _ (inr _) => False
+    | ftbd l__t =>
+      match t__s with
+      | tstop l__s _ | tsilent l__s => Stream.list_list_prefix l__t l__s
+      | tstream s__s => Stream.list_stream_prefix l__t s__s
+      end
+    end.
+
+  Definition rel : traceS -> traceT -> Prop :=
+    fun t__s t__t => t__s ≡ t__t \/ exists m, (t__t = tstop m OOM /\ prefixTS (ftbd m) t__s).
+  Hint Unfold rel.
+
+  Inductive syntactic_eq_finpref : finprefS -> finprefT -> Prop :=
+  | syntactic_eq_fstop : forall l e,
+      syntactic_eq_finpref (fstop l e) (fstop l ((inl e) : es endstateT))
+  | syntactic_eq_ftbd : forall l,
+      syntactic_eq_finpref (ftbd l) (ftbd l)
+  .
+
+  (* Definition rel_finpref : finprefS -> finprefT -> Prop := *)
+  (*   fun m__s m__t => syntactic_eq_finpref m__s m__t \/ exists l, (m__t = fstop l OOM /\ prefix_finpref (ftbd l) m__s). *)
+
+  Definition GC_traceT_traceS : Galois_Connection traceT traceS :=
+    induced_connection rel.
+
+  Definition τ : propS -> propT := α GC_traceT_traceS.
+  Lemma τ_def : forall πS t__t,
+      (τ πS) t__t <-> (exists t__s, t__s ≡ t__t /\ πS t__s) \/ (exists m t__s, t__t = tstop m OOM /\ prefixTS (ftbd m) t__s /\ πS t__s).
+  Proof.
+    intros πS t__t.
+    unfold τ, GC_traceT_traceS, induced_connection, low_rel; simpl.
+    split.
+    - intros H.
+      destruct H as [t__s [H1 H2]].
+      destruct H2 as [H2 | H2].
+      + left; eexists; split; eauto.
+      + destruct H2 as [m [H2 H3]]; subst.
+        right.
+        eexists; eexists; split; try split; eauto.
+    - intros H.
+      destruct H as [[t__s [H1 H2]] | [m [t__s [H1 [H2 H3]]]]].
+      + eexists; split; eauto.
+      + eexists; split; eauto.
+  Qed.
+
+  Definition σ : propT -> propS := γ GC_traceT_traceS.
+  Lemma σ_def : forall πT t__s,
+      (σ πT) t__s <-> (exists t__t, t__s ≡ t__t /\ πT t__t) /\ (forall m, prefixTS (ftbd m) t__s -> πT (tstop m OOM)).
+  Proof.
+    intros πT t__s.
+    unfold σ, GC_traceT_traceS, induced_connection, up_rel; simpl.
+    split.
+    - intros H.
+      split.
+      + destruct t__s.
+        * exists (tstop l (inl e : es endstateT)).
+          split; eauto.
+        * exists (tsilent l).
+          split; eauto.
+        * exists (tstream s).
+          split; eauto.
+      + intros m H0.
+        specialize (H (tstop m OOM)).
+        assert (rel t__s (tstop m OOM)).
+        { right.
+          exists m; split; auto. }
+        now apply H.
+    - intros H t__t H0.
+      destruct H as [[t__t' [H1 H2]] H3].
+      destruct H0.
+      + assert (t__t = t__t').
+        { clear -H H1.
+          inversion H; inversion H1; subst;
+            try now inversion H3.
+        }
+        now subst.
+      + destruct H as [m [H4 H5]]; subst; eauto.
+  Qed.
+
+
+  Lemma τ_preserves_dense : forall (π : propS),
+      Dense π -> Dense (τ π).
+  Proof.
+    unfold Dense, τ, GC_traceT_traceS, induced_connection, low_rel; simpl.
+    intros π HDense.
+    intros t__t Hfin.
+    destruct t__t as [l [e | []] | l | s].
+    - exists (tstop l e). split.
+      apply HDense. econstructor; eexists; eauto.
+      left; eauto.
+    - exists (tstop l (an_es endstateS)). split.
+      apply HDense. econstructor; eexists; eauto.
+      right; eexists; split; eauto.
+      clear; simpl; induction l.
+      reflexivity.
+      now split.
+    - destruct Hfin as [l' [e' Hn]].
+      inversion Hn.
+    - destruct Hfin as [l' [e' Hn]].
+      inversion Hn.
+  Qed.
+
+  Lemma σ_preserves_dense : forall (π : propT),
+      Dense π -> Dense (σ π).
+  Proof.
+    unfold Dense, σ, GC_traceT_traceS, induced_connection, up_rel; simpl.
+    intros π HDense.
+    intros t__s Hfin t__t Hrel.
+    destruct Hrel as [Hrel | Hrel].
+    - apply HDense; inversion Hrel; subst.
+      + now repeat eexists.
+      + destruct Hfin as [l' [e' Hn]].
+        inversion Hn.
+      + destruct Hfin as [l' [e' Hn]].
+        inversion Hn.
+    - destruct Hrel as [m [Heq Hpref]].
+      apply HDense.
+      rewrite Heq.
+      now repeat eexists.
+  Qed.
+
+
+  (* The goal is now to prove that τ and/or σ preserve Safety.
+   I need to define σ and τ for fprop, in order to use them
+   to transform the set of bad prefixes *)
+  Definition trace_TS (t__t : traceT) : traceS :=
+    match t__t with
+    | tstop l (inl e) => tstop l e
+    | tstop l (inr _) => tsilent l
+    | tsilent l => tsilent l
+    | tstream s => tstream s
+    end.
+
+  Lemma trace_TS_rel : forall (t__t : traceT),
+      rel (trace_TS t__t) t__t.
+  Proof.
+    destruct t__t as [l [e | []] | l | s];
+      try now left; constructor.
+    - right.
+      exists l.
+      split.
+      reflexivity.
+      now induction l; split.
+  Qed.
+
+  Definition finpref_ST (m__s : finprefS) : finprefT :=
+    match m__s with
+    | fstop l e => fstop l (inl e : es endstateT) : finprefT
+    | ftbd l => ftbd l
+    end.
+
+
+  Theorem τ_preserves_safety : forall (π : propS),
+      Safety π -> Safety (τ π).
+  Proof.
+    unfold Safety, τ, GC_traceT_traceS, induced_connection, low_rel; simpl.
+    intros π Hsafety t__t Ht.
+    rewrite not_ex_forall_not in Ht;
+      setoid_rewrite de_morgan1 in Ht;
+      setoid_rewrite or_comm in Ht;
+      setoid_rewrite <- imp_equiv in Ht.
+    specialize (Hsafety (trace_TS t__t) (Ht (trace_TS t__t) (trace_TS_rel t__t))).
+    destruct Hsafety as [m [Hpref H]].
+    exists (finpref_ST m).
+    split.
+    - destruct m as [l e | l];
+        destruct t__t as [l' [e' | []] | l' | s'];
+        try now auto.
+      now inversion Hpref; subst.
+    - intros t__t' Hpref'.
+      rewrite not_ex_forall_not;
+        setoid_rewrite de_morgan1;
+        setoid_rewrite or_comm;
+        setoid_rewrite <- imp_equiv.
+      intros t__s Hrel.
+      apply H.
+      destruct m as [l e | l].
+      + destruct t__t' as [l' [e' | []] | l' | s'];
+          try now auto.
+        * destruct Hrel as [Hrel | Hrel].
+          -- destruct t__s as [l'' e'' | l'' | s''];
+               try now auto.
+             inversion Hrel; subst.
+             now inversion Hpref' as [H0 H1]; inversion H0; subst.
+          -- destruct Hrel as [m [H1 H2]].
+             now inversion H1.
+        * destruct Hpref' as [H1 H2]; now inversion H1.
+      + destruct t__t' as [l' [e' | []] | l' | s'];
+          try now auto.
+        * destruct Hrel as [Hrel | Hrel].
+          -- destruct t__s as [l'' e'' | l'' | s''];
+               try now auto.
+             inversion Hrel; subst.
+             now assumption.
+          -- destruct Hrel as [m [H1 H2]].
+             now inversion H1.
+        * destruct Hrel as [Hrel | Hrel].
+          -- destruct t__s as [l'' e'' | l'' | s''];
+               try now auto.
+          -- destruct Hrel as [m [H1 H2]]; try now auto.
+             inversion H1; subst.
+             simpl in Hpref'.
+             destruct t__s as [l'' e'' | l'' | s''];
+               try now eapply Stream.list_list_prefix_trans; eassumption.
+             simpl in *.
+             { clear -Hpref' H2.
+               generalize dependent s''. generalize dependent m.
+               induction l as [| e l]; intros m Hlm s Hms.
+               - reflexivity.
+               - destruct m as [| e' l'];
+                   destruct Hlm;
+                   subst.
+                 destruct s as [e s].
+                 simpl in *.
+                 destruct Hms as [? Hl's]; subst.
+                 split; first reflexivity.
+                 now eapply IHl; eassumption.
+             }
+        * destruct Hrel as [Hrel | Hrel].
+          -- destruct t__s as [l'' e'' | l'' | s''];
+               try now auto.
+             inversion Hrel; subst.
+             assumption.
+          -- destruct Hrel as [m [H1 H2]];
+               try now auto.
+        * destruct Hrel as [Hrel | Hrel].
+          -- destruct t__s as [l'' e'' | l'' | s''];
+               try now auto.
+             inversion Hrel; subst.
+             assumption.
+          -- destruct Hrel as [m [H1 H2]];
+               try now auto.
+  Qed.
+
+  Definition finpref_TS (m__t : finprefT) : finprefS :=
+    match m__t with
+    | fstop l (inl e) => fstop l e
+    | fstop l (inr e) => ftbd l
+    | ftbd l => ftbd l
+    end.
+
+  Definition trace_ST (t__s : traceS) : traceT :=
+    match t__s with
+    | tstop l e => tstop l (inl e : es endstateT)
+    (* | tstop l e => tstop l OOM *)
+    | tsilent l => tsilent l
+    | tstream s => tstream  s
+    end.
+
+  Lemma rel_target_terminating (t__S : traceS)
+        (l : list (ev event))
+        (e : es endstate):
+    rel t__S ((@tstop event endstateT l) ((inl out_of_memory e))) ->
+    t__S = (@tstop event endstateS l e).
+  Proof.
+    destruct t__S; eauto; intros [rel_by_eq | [m [H1 H2]]];
+      try now inversion rel_by_eq.
+    + subst. now induction l.
+    + now inversion H1.
+    + now inversion H1.
+  Qed.
+
+  Lemma rel_tstop_OOM (l : list (ev event))
+        (e : es endstateS):
+    rel (tstop l e) (tstop l OOM).
+  Proof.
+    right. exists l. split; auto.
+    now induction l.
+  Qed.
+
+  Lemma σ_preserves_safety : forall (π : propT),
+      Safety π -> Safety (σ π).
+  Proof.
+    intros π__T safety_π__T t__S not_t__S.
+    unfold σ, γ in not_t__S. simpl in not_t__S. unfold up_rel in not_t__S.
+    rewrite not_forall_ex_not in not_t__S.
+    destruct not_t__S as [t__T not_t__S]. rewrite not_imp in not_t__S.
+    destruct not_t__S as [rel_ts_tt not_t__T].
+    destruct (safety_π__T t__T not_t__T) as [m__T [pref_mt_tt mt_wit]].
+    destruct m__T.
+    + destruct es.
+      ++ destruct t__T; inversion pref_mt_tt.
+         apply prefix_stop_terminating_trace in pref_mt_tt.
+         subst.
+         assert (t__S = tstop l0 e) by now apply rel_target_terminating.
+         subst.
+         exists (fstop l0 e). split; try now auto.
+         intros t__S' pref_m_t__S'.
+         unfold σ, γ. simpl.  unfold up_rel. rewrite not_forall_ex_not.
+         exists (@tstop event endstateT l0 (inl out_of_memory e)).
+         rewrite not_imp. split; auto.
+         apply prefix_stop_terminating_trace in pref_m_t__S'. now subst.
+      ++ destruct t__T; inversion pref_mt_tt. subst.
+         destruct rel_ts_tt as [Heq | [m [H1 H2]]].
+         +++ inversion Heq.
+         +++ rewrite H1 in *.
+             exists (ftbd m). split; auto.
+             intros t__S' Hpref'.  unfold σ, γ. simpl.  unfold up_rel. rewrite not_forall_ex_not.
+             exists (tstop m OOM). rewrite not_imp.
+             split; auto. right. now (exists m).
+    + assert (prefix (ftbd l) (tstop l OOM)).
+      { simpl; now apply  list_list_prefix_ref. }
+      specialize (mt_wit (tstop l OOM) H).
+      exists (ftbd l). split.
+      ++ destruct rel_ts_tt as  [Heq | [m [H1 H2]]].
+         +++ inversion Heq; subst; now simpl in *.
+         +++ subst. destruct t__S; simpl in *.
+             eapply list_list_prefix_trans. exact pref_mt_tt. exact H2.
+             eapply list_list_prefix_trans. exact pref_mt_tt. exact H2.
+             eapply list_stream_prefix_trans. exact pref_mt_tt. exact H2.
+      ++ intros t__S' Hpref'.  unfold σ, γ. simpl.  unfold up_rel. rewrite not_forall_ex_not.
+         exists (tstop l OOM). rewrite not_imp.
+         split; auto. right. now exists l.
+  Qed.
+
+End ResourceExhaustion.
