ResourceExhaustion/Machine.v
@@ -1,0 +1,355 @@
+Require Import Bool Arith Omega List Coq.Program.Equality.
+Require Import Maps Imp.
+Require Import List.
+Import ListNotations.
+Require Import Sequences.
+Require Import TraceModel.
+
+
+Set Bullet Behavior "Strict Subproofs".
+(** This chapter defines a compiler from the Imp language to a virtual machine
+  (a small subset of the Java Virtual Machine) and proves that this
+  compiler preserves the semantics of the source programs. *)
+
+(** * 1. The virtual machine. *)
+
+(** The machine operates on a code [c] (a fixed list of instructions)
+  and three variable components:
+- a program counter, denoting a position in [c]
+- a state assigning integer values to variables
+- an evaluation stack, containing integers.
+*)
+
+(** The instruction set of the machine. *)
+
+Inductive instruction: Type :=
+  | Iconst(n: nat)                 (**r push integer [n] on stack *)
+  | Ivar(x: id)                    (**r push the value of variable [x] *)
+  | Isetvar(x: id)                 (**r pop an integer, assign it to variable [x] *)
+  | Iadd                           (**r pop [n2], pop [n1], push back [n1+n2] *)
+  | Isub                           (**r pop [n2], pop [n1], push back [n1-n2] *)
+  | Imul                           (**r pop [n2], pop [n1], push back [n1*n2] *)
+  | Ibranch_forward(ofs: nat)      (**r skip [ofs] instructions forward *)
+  | Ibranch_backward(ofs: nat)     (**r skip [ofs] instructions backward *)
+  | Ibeq(ofs: nat)                 (**r pop [n2], pop [n1], skip [ofs] forward if [n1=n2] *)
+  | Ibne(ofs: nat)                 (**r pop [n2], pop [n1], skip [ofs] forward if [n1<>n2] *)
+  | Ible(ofs: nat)                 (**r pop [n2], pop [n1], skip [ofs] forward if [n1<=n2] *)
+  | Ibgt(ofs: nat)                 (**r pop [n2], pop [n1], skip [ofs] forward if [n1>n2] *)
+  | Iout                         (**r pop an integer, outputs it *)
+  | Ihalt.                         (**r terminate execution successfully *)
+
+Definition code := list instruction.
+
+(** [code_at C pc = Some i] if [i] is the instruction at position [pc]
+  in the list of instructions [C]. *)
+
+Fixpoint code_at (C: code) (pc: nat) : option instruction :=
+  match C, pc with
+  | nil, _ => None
+  | i :: C', O => Some i
+  | i :: C', S pc' => code_at C' pc'
+  end.
+
+Definition stack := list nat.
+
+(** The semantics of the virtual machine is given in small-step style,
+  as a transition relation between machine configuration: triples
+  (program counter, evaluation stack, variable state).
+  The transition relation is parameterized by the code [c].
+  There is one transition rule for each kind of instruction,
+  except [Ihalt], which has no transition. *)
+
+Definition configuration := (nat * stack * state)%type.
+
+Inductive transition (C: code): configuration -> list (nat) -> configuration -> Prop :=
+  | trans_const: forall pc stk s n,
+      code_at C pc = Some(Iconst n) ->
+      transition C (pc, stk, s) [] (pc + 1, n :: stk, s)
+  | trans_var: forall pc stk s x,
+      code_at C pc = Some(Ivar x) ->
+      transition C (pc, stk, s) [] (pc + 1, s x :: stk, s)
+  | trans_out: forall pc stk s n,
+      code_at C pc = Some Iout ->
+      transition C (pc, n :: stk, s) [n] (pc + 1, stk, s)
+  | trans_setvar: forall pc stk s x n,
+      code_at C pc = Some(Isetvar x) ->
+      transition C (pc, n :: stk, s) [] (pc + 1, stk, t_update s x n)
+  | trans_add: forall pc stk s n1 n2,
+      code_at C pc = Some(Iadd) ->
+      transition C (pc, n2 :: n1 :: stk, s) [] (pc + 1, (n1 + n2) :: stk, s)
+  | trans_sub: forall pc stk s n1 n2,
+      code_at C pc = Some(Isub) ->
+      transition C (pc, n2 :: n1 :: stk, s) [] (pc + 1, (n1 - n2) :: stk, s)
+  | trans_mul: forall pc stk s n1 n2,
+      code_at C pc = Some(Imul) ->
+      transition C (pc, n2 :: n1 :: stk, s) [] (pc + 1, (n1 * n2) :: stk, s)
+  | trans_branch_forward: forall pc stk s ofs pc',
+      code_at C pc = Some(Ibranch_forward ofs) ->
+      pc' = pc + 1 + ofs ->
+      transition C (pc, stk, s) [] (pc', stk, s)
+  | trans_branch_backward: forall pc stk s ofs pc',
+      code_at C pc = Some(Ibranch_backward ofs) ->
+      pc' = pc + 1 - ofs ->
+      transition C (pc, stk, s) [] (pc', stk, s)
+  | trans_beq: forall pc stk s ofs n1 n2 pc',
+      code_at C pc = Some(Ibeq ofs) ->
+      pc' = (if beq_nat n1 n2 then pc + 1 + ofs else pc + 1) ->
+      transition C (pc, n2 :: n1 :: stk, s) [] (pc', stk, s)
+  | trans_bne: forall pc stk s ofs n1 n2 pc',
+      code_at C pc = Some(Ibne ofs) ->
+      pc' = (if beq_nat n1 n2 then pc + 1 else pc + 1 + ofs) ->
+      transition C (pc, n2 :: n1 :: stk, s) [] (pc', stk, s)
+  | trans_ble: forall pc stk s ofs n1 n2 pc',
+      code_at C pc = Some(Ible ofs) ->
+      pc' = (if leb n1 n2 then pc + 1 + ofs else pc + 1) ->
+      transition C (pc, n2 :: n1 :: stk, s) [] (pc', stk, s)
+  | trans_bgt: forall pc stk s ofs n1 n2 pc',
+      code_at C pc = Some(Ibgt ofs) ->
+      pc' = (if leb n1 n2 then pc + 1 else pc + 1 + ofs) ->
+      transition C (pc, n2 :: n1 :: stk, s) [] (pc', stk, s).
+
+(** As usual with small-step semantics, we form sequences of machine transitions
+  to define the behavior of a code.  We always start with [pc = 0]
+  and an empty evaluation stack.  We stop successfully if [pc] points
+  to an [Ihalt] instruction and the evaluation stack is empty.
+
+  If [R] is a binary relation, [star R] is its reflexive transitive closure.
+  (See file [Sequences] for the definition.)  [star (transition C)]
+  therefore represents a sequence of  zero, one or several machine transitions.
+*)
+
+Definition mach_terminates (C: code) (s_init s_fin: state) l :=
+  exists pc,
+  code_at C pc = Some Ihalt /\
+  star (transition C) (0, nil, s_init) l (pc, nil, s_fin).
+
+(** Likewise, [infseq R] represents an infinite sequence of [R] transitions.
+  (Also defined in file [Sequences].) *)
+
+Definition mach_diverges (C: code) (s_init: state) s :=
+  infseq (transition C) s (0, nil, s_init).
+
+Definition mach_reacts (C: code) (s_init: state) s :=
+  infseq_prod (transition C) s (0, nil, s_init).
+
+Definition mach_silent (C : code) (s_init s_fin: state) l :=
+  exists pc stack,
+    star (transition C) (0, nil, s_init) l (pc, stack, s_fin) /\
+    infseq_silent (transition C) (pc, stack, s_fin).
+
+(** A third case can occur: after a finite number of transitions,
+  the machine hits a configuration where it cannot make any transition,
+  and this state is not a final configuration ([Ihalt] instruction and empty stack).
+  In this case, we say that the machine "goes wrong", which is
+  a politically-correct way of saying that our program just crashed. *)
+
+Definition mach_goes_wrong (C: code) (s_init: state) l :=
+  exists pc, exists stk, exists s_fin,
+  star (transition C) (0, nil, s_init) l (pc, stk, s_fin)
+  /\ irred (transition C) (pc, stk, s_fin)
+  /\ (code_at C pc <> Some Ihalt \/ stk <> nil).
+
+(** An important property of the virtual machine is that it is deterministic:
+  from a given configuration, it can transition to at most one other configuration. *)
+
+Lemma machine_deterministic:
+  forall C config config1 config2 e1 e2,
+  transition C config e1 config1 -> transition C config e2 config2 -> config1 = config2 /\ e1 = e2.
+Proof.
+  intros. inversion H; subst; inversion H0; split; try congruence.
+  destruct (beq_nat n1 n2); congruence.
+  destruct (beq_nat n1 n2); congruence.
+  destruct (leb n1 n2); congruence.
+  destruct (leb n1 n2); congruence.
+Qed.
+
+Lemma machine_deterministic_config:
+  forall C config config1 config2 e1 e2,
+    transition C config e1 config1 -> transition C config e2 config2 -> config1 = config2.
+Proof.
+  intros C config config1 config2 e1 e2 H H0.
+  now destruct (machine_deterministic _ _ _ _ _ _ H H0).
+Qed.
+
+Lemma machine_deterministic_event:
+  forall C config config1 config2 e1 e2,
+    transition C config e1 config1 -> transition C config e2 config2 -> e1 = e2.
+Proof.
+  intros C config config1 config2 e1 e2 H H0.
+  now destruct (machine_deterministic _ _ _ _ _ _ H H0).
+Qed.
+
+(** As a consequence of this determinism, it follows that
+  the final state of a terminating program is unique,
+  and that a program cannot both terminate and diverge,
+  or terminate and go wrong, or diverge and go wrong.
+  These results follow from the generic determinism properties 
+  found at the end of module [Sequence]. *)
+
+Remark stop_irred:
+  forall C pc stk st,
+  code_at C pc = Some Ihalt -> irred (transition C) (pc, stk, st).
+Proof.
+  unfold irred; intros. unfold not; intros. inversion H0; congruence.
+Qed.
+
+Lemma terminates_unique:
+  forall C st st1 st2 l1 l2, mach_terminates C st st1 l1 -> mach_terminates C st st2 l2 -> st1 = st2 /\ l1 = l2.
+Proof.
+  unfold mach_terminates; intros. destruct H as (pc1 & A1 & B1), H0 as (pc2 & A2 & B2).
+  assert (((pc1, nil, st1) : configuration) = ((pc2, nil, st2) : configuration)).
+  { eapply finseq_unique; eauto using machine_deterministic, stop_irred. }
+  assert (l1 = l2).
+  { eapply finseq_unique; eauto using machine_deterministic, stop_irred. }
+  split; congruence.
+Qed.
+
+Lemma goeswrong_unique:
+  forall C st l1 l2, mach_goes_wrong C st l1 -> mach_goes_wrong C st l2 -> l1 = l2.
+Proof.
+  unfold mach_goes_wrong; intros C st l1 l2 H H0.
+  destruct H as (pc1 & stk1 & s_fin1 & H1 & H1' & H1'').
+  destruct H0 as (pc2 & stk2 & s_fin2 & H2 & H2' & H2'').
+  eapply finseq_unique; eauto using machine_deterministic, stop_irred.
+Qed.
+
+Lemma silent_unique:
+  forall C st st1 st2 l1 l2, mach_silent C st st1 l1 -> mach_silent C st st2 l2 -> l1 = l2.
+Proof.
+  unfold mach_silent; intros C st st1 st2 l1 l2 H H0.
+  destruct H as (pc1 & stk1 & Hstar1 & H1 ).
+  destruct H0 as (pc2 & stk2 & Hstar2 & H2 ).
+  pose proof (star_star_inv (machine_deterministic C) Hstar1 Hstar2)
+    as [[l [Hinv1 Hinv2]] | [l [Hinv1 Hinv2]]]; subst.
+  pose proof (infseq_silent_star_inv (machine_deterministic C) Hinv2 H2)
+    as [Hinv1' Hinv2'].
+  subst; now apply app_nil_r.
+  pose proof (infseq_silent_star_inv (machine_deterministic C) Hinv2 H1)
+    as [Hinv1' Hinv2'].
+  subst; now rewrite app_nil_r.
+Qed.
+
+CoInductive stream_eq' {A : Type} : @Stream.stream A -> @Stream.stream A -> Prop :=
+  eq'_scons : forall l s1 s2,
+    l <> [] -> stream_eq' s1 s2 -> stream_eq' (Stream.app_list_stream l s1) (Stream.app_list_stream l s2).
+
+Lemma reacts_unique:
+  forall C st s1 s2, mach_reacts C st s1 -> mach_reacts C st s2 -> Stream.stream_eq s1 s2.
+Proof.
+  assert (reacts_unique' : forall C a s1 s2, infseq_prod (transition C) s1 a -> infseq_prod (transition C) s2 a -> stream_eq' s1 s2).
+  cofix Hfix; intros.
+  inversion H; subst; clear H. inversion H0; subst; clear H0.
+  pose proof (infseq_prod_inv).
+  specialize (H0 _ _ _ (machine_deterministic C) _ _ _ H1 _ _ _ _ H H2 H4 H3 H5).
+  destruct H0 as [a' [l1 [s1' [s2' [H11 [H12 [H13 [H14 H15]]]]]]]]; auto.
+  rewrite H14; rewrite H15.
+  econstructor; eauto.
+  assert (forall A s1 s2, @stream_eq' A s1 s2 -> Stream.stream_eq s1 s2).
+  {
+    cofix Hfix. intros A s1 s2 H.
+    inversion H; subst; clear H.
+    destruct l. congruence.
+    simpl.
+    destruct l. simpl. constructor. apply Hfix. auto.
+    constructor. apply Hfix. constructor. congruence.
+    assumption.
+  }
+  intros C st s1 s2 H0 H1.
+  unfold mach_reacts in *.
+  apply H. eapply reacts_unique'; eauto.
+Qed.
+
+Lemma terminates_goeswrong_exclusive:
+  forall C st st' l l', mach_terminates C st st' l -> mach_goes_wrong C st l' -> False.
+Proof.
+  unfold mach_terminates, mach_goes_wrong; intros.
+  destruct H as (pc1 & A1 & B1), H0 as (pc2 & stk2 & st2 & A2 & B2 & C2).
+  assert (((pc1, nil, st') : configuration) = ((pc2, stk2, st2) : configuration)).
+  { eapply finseq_unique; eauto using machine_deterministic, stop_irred. }
+  inversion H. subst pc2 stk2 st2. destruct C2; congruence.
+Qed.
+
+Lemma terminates_diverges_exclusive:
+  forall C st st' l s, mach_terminates C st st' l -> mach_diverges C st s -> False.
+Proof.
+  unfold mach_terminates, mach_diverges; intros.
+  destruct H as (pc1 & A1 & B1).
+  eapply infseq_finseq_excl with (R := transition C); eauto using machine_deterministic, stop_irred.
+Qed.
+
+
+Lemma terminates_reacts_exclusive:
+  forall C st st' l s, mach_terminates C st st' l -> mach_reacts C st s -> False.
+Proof.
+  unfold mach_terminates, mach_reacts; intros.
+  destruct H as (pc1 & A1 & B1).
+  eapply infseq_finseq_excl with (R := transition C); eauto using machine_deterministic, stop_irred.
+  eapply infseq_prod_infseq; eauto.
+Qed.
+
+Lemma goeswrong_diverges_exclusive:
+  forall C st l s, mach_goes_wrong C st l -> mach_diverges C st s -> False.
+Proof.
+  unfold mach_terminates, mach_diverges; intros. 
+  destruct H as (pc2 & stk2 & st2 & A2 & B2 & C2).
+  eapply infseq_finseq_excl with (R := transition C); eauto using machine_deterministic, stop_irred.
+Qed.
+
+Lemma goeswrong_silent_exclusive:
+  forall C st st' l l', mach_goes_wrong C st l -> mach_silent C st st' l' -> False.
+Proof.
+  intros C st st' l l' H H0.
+  destruct H as [pc [s_fin [H1 H2]]].
+  destruct H0 as [pc' [stk' [H1' H2']]].
+  eapply infseq_silent_finseq_excl.
+  eauto using machine_deterministic.
+  eauto. eapply H2. eauto. eauto using stop_irred.
+  destruct H2 as [A1 [A2 A3]].
+  eapply A2.
+Qed.
+
+Lemma goeswrong_reacts_exclusive:
+  forall C st l s, mach_goes_wrong C st l -> mach_reacts C st s -> False.
+Proof.
+  unfold mach_terminates, mach_reacts; intros.
+  destruct H as [pc [s_fin [H1 [H2 [H3 H4]]]]].
+  eapply infseq_finseq_excl.
+  eauto using machine_deterministic.
+  eauto. eapply H3.
+  eapply infseq_prod_infseq; eauto.
+Qed.
+
+Lemma terminates_silent_exclusive:
+  forall C st st' st'' l l', mach_terminates C st st' l -> mach_silent C st st'' l' -> False.
+Proof.
+  unfold mach_terminates, mach_silent; intros.
+  destruct H as [pc [H1 H2]].
+  destruct H0 as [pc' [stk' [H1' H2']]].
+  eapply infseq_silent_finseq_excl.
+  eauto using machine_deterministic.
+  eauto. eapply H2. eauto. eauto using stop_irred.
+Qed.
+
+(* Lemma silent_diverges_exclusive: *)
+(*   forall C st st' l s, mach_diverges C st s -> mach_silent C st st' l -> False. *)
+(* Proof. *)
+(*   unfold mach_diverges, mach_silent; intros. *)
+(*   destruct H0 as [pc [stk [H1 H2]]]. *)
+(*   (* eapply infseq_silent_excl. *) *)
+(*   eauto using machine_deterministic. *)
+(* Admitted. *)
+
+
+Lemma silent_reacts_exclusive:
+  forall C st st' s l,
+    mach_reacts C st s -> mach_silent C st st' l -> False.
+Proof.
+  intros C st st' s l H H0.
+  destruct H0 as [pc [stk [H0 H1]]].
+  (* inversion H; subst; clear H. *)
+  pose proof (star_infseq_prod_inv (machine_deterministic C) H0 H)
+    as [s' [H2 H3]].
+  inversion H2; subst; clear H2.
+  pose proof (infseq_silent_star_inv (machine_deterministic C) H4 H1).
+  destruct H2; now congruence.
+Qed.
