ResourceExhaustion/MachineStackLimited.v
@@ -1,0 +1,339 @@
+Require Import Bool Arith Omega List Coq.Program.Equality.
+Require Import Maps Imp.
+Require Import List.
+Import ListNotations.
+Require Import Sequences.
+Require Import TraceModel.
+Require Import Machine.
+
+Set Bullet Behavior "Strict Subproofs".
+
+
+Definition stack_limit := 50.
+
+Definition configuration_limited := option configuration.
+Inductive transition_limited (C : code) : configuration_limited -> list nat -> configuration_limited -> Prop :=
+| transition_OOM : forall pc1 stk1 st1 pc2 stk2 st2 l,
+    transition C (pc1, stk1, st1) l (pc2, stk2, st2) ->
+    stack_limit <= List.length stk2 ->
+    transition_limited C (Some (pc1, stk1, st1)) [] None
+| transition_some : forall pc1 stk1 st1 pc2 stk2 st2 l,
+    transition C (pc1, stk1, st1) l (pc2, stk2, st2) ->
+    List.length stk2 < stack_limit ->
+    transition_limited C (Some (pc1, stk1, st1)) l (Some (pc2, stk2, st2)).
+
+(** As usual with small-step semantics, we form sequences of machine transitions
+  to define the behavior of a code.  We always start with [pc = 0]
+  and an empty evaluation stack.  We stop successfully if [pc] points
+  to an [Ihalt] instruction and the evaluation stack is empty.
+
+  If [R] is a binary relation, [star R] is its reflexive transitive closure.
+  (See file [Sequences] for the definition.)  [star (transition_limited C)]
+  therefore represents a sequence of  zero, one or several machine transition_limiteds.
+*)
+
+Definition mach_terminates (C: code) (s_init s_fin: state) l :=
+  exists pc,
+  code_at C pc = Some Ihalt /\
+  star (transition_limited C) (Some (0, nil, s_init)) l (Some (pc, nil, s_fin)).
+
+Definition mach_OOM (C : code) (s_init : state) l :=
+    star (transition_limited C) (Some (0, nil, s_init)) l None.
+
+(** Likewise, [infseq R] represents an infinite sequence of [R] transition_limiteds.
+  (Also defined in file [Sequences].) *)
+
+Definition mach_diverges (C: code) (s_init: state) s :=
+  infseq (transition_limited C) s (Some (0, nil, s_init)).
+
+Definition mach_reacts (C: code) (s_init: state) s :=
+  infseq_prod (transition_limited C) s (Some (0, nil, s_init)).
+
+Definition mach_silent (C : code) (s_init s_fin: state) l :=
+  exists pc stack,
+    star (transition_limited C) (Some (0, nil, s_init)) l (Some (pc, stack, s_fin)) /\
+    infseq_silent (transition_limited C) (Some (pc, stack, s_fin)).
+
+(** A third case can occur: after a finite number of transition_limiteds,
+  the machine hits a configuration_limited where it cannot make any transition_limited,
+  and this state is not a final configuration_limited ([Ihalt] instruction and empty stack).
+  In this case, we say that the machine "goes wrong", which is
+  a politically-correct way of saying that our program just crashed. *)
+
+Definition mach_goes_wrong (C: code) (s_init: state) l :=
+  exists pc, exists stk, exists s_fin,
+  star (transition_limited C) (Some (0, nil, s_init)) l (Some (pc, stk, s_fin))
+  /\ irred (transition_limited C) (Some (pc, stk, s_fin))
+  /\ (code_at C pc <> Some Ihalt \/ stk <> nil).
+
+(** An important property of the virtual machine is that it is deterministic:
+  from a given configuration_limited, it can transition_limited to at most one other configuration_limited. *)
+
+Lemma machine_deterministic:
+  forall C config config1 config2 e1 e2,
+  transition_limited C config e1 config1 -> transition_limited C config e2 config2 -> config1 = config2 /\ e1 = e2.
+Proof.
+  intros.
+  inversion H; inversion H0; subst; split; try congruence;
+    match goal with
+    | Heq: Some _ = Some _ |- _ => inversion Heq; subst; clear Heq
+    end;
+  (repeat match goal with
+            | Htrans: transition _ _ _ _ |- _ => inversion Htrans; subst; clear Htrans
+            end);
+    try congruence;
+  match goal with
+  | Heq1 : code_at _ _ = Some _, Heq2 : code_at _ _ = Some _ |- _ =>
+    rewrite Heq1 in Heq2; inversion Heq2; subst; clear Heq2
+  end;
+     try omega.
+  destruct (beq_nat n1 n2); congruence.
+  destruct (beq_nat n1 n2); congruence.
+  destruct (leb n1 n2); congruence.
+  destruct (leb n1 n2); congruence.
+Qed.
+
+Lemma machine_deterministic_config:
+  forall C config config1 config2 e1 e2,
+    transition_limited C config e1 config1 -> transition_limited C config e2 config2 -> config1 = config2.
+Proof.
+  intros C config config1 config2 e1 e2 H H0.
+  now destruct (machine_deterministic _ _ _ _ _ _ H H0).
+Qed.
+
+Lemma machine_deterministic_event:
+  forall C config config1 config2 e1 e2,
+    transition_limited C config e1 config1 -> transition_limited C config e2 config2 -> e1 = e2.
+Proof.
+  intros C config config1 config2 e1 e2 H H0.
+  now destruct (machine_deterministic _ _ _ _ _ _ H H0).
+Qed.
+
+(** As a consequence of this determinism, it follows that
+  the final state of a terminating program is unique,
+  and that a program cannot both terminate and diverge,
+  or terminate and go wrong, or diverge and go wrong.
+  These results follow from the generic determinism properties 
+  found at the end of module [Sequence]. *)
+
+Remark stop_irred:
+  forall C pc stk st,
+  code_at C pc = Some Ihalt -> irred (transition_limited C) (Some (pc, stk, st)).
+Proof.
+  unfold irred; intros. unfold not; intros.
+  inversion H0 as [? ? ? ? ? ? ? Htrans| ? ? ? ? ? ? ? Htrans]; subst;
+    inversion Htrans; congruence.
+Qed.
+
+Lemma terminates_unique:
+  forall C st st1 st2 l1 l2, mach_terminates C st st1 l1 -> mach_terminates C st st2 l2 -> st1 = st2 /\ l1 = l2.
+Proof.
+  unfold mach_terminates; intros. destruct H as (pc1 & A1 & B1), H0 as (pc2 & A2 & B2).
+  assert ((Some (pc1, nil, st1) : configuration_limited) = (Some (pc2, nil, st2) : configuration_limited)).
+  { eapply finseq_unique; eauto using machine_deterministic, stop_irred. }
+  assert (l1 = l2).
+  { eapply finseq_unique; eauto using machine_deterministic, stop_irred. }
+  split; congruence.
+Qed.
+
+Lemma goeswrong_unique:
+  forall C st l1 l2, mach_goes_wrong C st l1 -> mach_goes_wrong C st l2 -> l1 = l2.
+Proof.
+  unfold mach_goes_wrong; intros C st l1 l2 H H0.
+  destruct H as (pc1 & stk1 & s_fin1 & H1 & H1' & H1'').
+  destruct H0 as (pc2 & stk2 & s_fin2 & H2 & H2' & H2'').
+  eapply finseq_unique; eauto using machine_deterministic, stop_irred.
+Qed.
+
+Lemma OOM_unique:
+  forall C st l1 l2, mach_OOM C st l1 -> mach_OOM C st l2 -> l1 = l2.
+Proof.
+  unfold mach_OOM; intros C st l1 l2 H H0.
+  eapply finseq_unique; eauto using machine_deterministic;
+    intros c l Hn; inversion Hn.
+Qed.
+
+Lemma silent_unique:
+  forall C st st1 st2 l1 l2, mach_silent C st st1 l1 -> mach_silent C st st2 l2 -> l1 = l2.
+Proof.
+  unfold mach_silent; intros C st st1 st2 l1 l2 H H0.
+  destruct H as (pc1 & stk1 & Hstar1 & H1 ).
+  destruct H0 as (pc2 & stk2 & Hstar2 & H2 ).
+  pose proof (star_star_inv (machine_deterministic C) Hstar1 Hstar2)
+    as [[l [Hinv1 Hinv2]] | [l [Hinv1 Hinv2]]]; subst.
+  pose proof (infseq_silent_star_inv (machine_deterministic C) Hinv2 H2)
+    as [Hinv1' Hinv2'].
+  subst; now apply app_nil_r.
+  pose proof (infseq_silent_star_inv (machine_deterministic C) Hinv2 H1)
+    as [Hinv1' Hinv2'].
+  subst; now rewrite app_nil_r.
+Qed.
+
+CoInductive stream_eq' {A : Type} : @Stream.stream A -> @Stream.stream A -> Prop :=
+  eq'_scons : forall l s1 s2,
+    l <> [] -> stream_eq' s1 s2 -> stream_eq' (Stream.app_list_stream l s1) (Stream.app_list_stream l s2).
+
+Lemma reacts_unique:
+  forall C st s1 s2, mach_reacts C st s1 -> mach_reacts C st s2 -> Stream.stream_eq s1 s2.
+Proof.
+  assert (reacts_unique' : forall C a s1 s2, infseq_prod (transition_limited C) s1 a -> infseq_prod (transition_limited C) s2 a -> stream_eq' s1 s2).
+  cofix Hfix; intros.
+  inversion H; subst; clear H. inversion H0; subst; clear H0.
+  pose proof (infseq_prod_inv).
+  specialize (H0 _ _ _ (machine_deterministic C) _ _ _ H1 _ _ _ _ H H2 H4 H3 H5).
+  destruct H0 as [a' [l1 [s1' [s2' [H11 [H12 [H13 [H14 H15]]]]]]]]; auto.
+  rewrite H14; rewrite H15.
+  econstructor; eauto.
+  assert (forall A s1 s2, @stream_eq' A s1 s2 -> Stream.stream_eq s1 s2).
+  {
+    cofix Hfix. intros A s1 s2 H.
+    inversion H; subst; clear H.
+    destruct l. congruence.
+    simpl.
+    destruct l. simpl. constructor. apply Hfix. auto.
+    constructor. apply Hfix. constructor. congruence.
+    assumption.
+  }
+  intros C st s1 s2 H0 H1.
+  unfold mach_reacts in *.
+  apply H. eapply reacts_unique'; eauto.
+Qed.
+
+Lemma terminates_goeswrong_exclusive:
+  forall C st st' l l', mach_terminates C st st' l -> mach_goes_wrong C st l' -> False.
+Proof.
+  unfold mach_terminates, mach_goes_wrong; intros.
+  destruct H as (pc1 & A1 & B1), H0 as (pc2 & stk2 & st2 & A2 & B2 & C2).
+  assert ((Some (pc1, nil, st') : configuration_limited) = (Some (pc2, stk2, st2) : configuration_limited)).
+  { eapply finseq_unique; eauto using machine_deterministic, stop_irred. }
+  inversion H. subst pc2 stk2 st2. destruct C2; congruence.
+Qed.
+
+Lemma terminates_OOM_exclusive:
+  forall C st st' l l', mach_terminates C st st' l -> mach_OOM C st l' -> False.
+Proof.
+  unfold mach_terminates, mach_OOM; intros.
+  destruct H as (pc1 & A1 & B1). (* H0 as (pc2 & stk2 & st2 & A2 & B2 & C2). *)
+  assert ((Some (pc1, nil, st') : configuration_limited) = (None : configuration_limited)).
+  { eapply finseq_unique; eauto using machine_deterministic, stop_irred.
+    unfold irred.  intros b l'' Hn. inversion Hn. }
+  congruence.
+Qed.
+
+Lemma terminates_diverges_exclusive:
+  forall C st st' l s, mach_terminates C st st' l -> mach_diverges C st s -> False.
+Proof.
+  unfold mach_terminates, mach_diverges; intros.
+  destruct H as (pc1 & A1 & B1).
+  eapply infseq_finseq_excl with (R := transition_limited C); eauto using machine_deterministic, stop_irred.
+Qed.
+
+Lemma terminates_reacts_exclusive:
+  forall C st st' l s, mach_terminates C st st' l -> mach_reacts C st s -> False.
+Proof.
+  unfold mach_terminates, mach_reacts; intros.
+  destruct H as (pc1 & A1 & B1).
+  eapply infseq_finseq_excl with (R := transition_limited C); eauto using machine_deterministic, stop_irred.
+  eapply infseq_prod_infseq; eauto.
+Qed.
+
+Lemma goeswrong_diverges_exclusive:
+  forall C st l s, mach_goes_wrong C st l -> mach_diverges C st s -> False.
+Proof.
+  unfold mach_terminates, mach_diverges; intros. 
+  destruct H as (pc2 & stk2 & st2 & A2 & B2 & C2).
+  eapply infseq_finseq_excl with (R := transition_limited C); eauto using machine_deterministic, stop_irred.
+Qed.
+
+Lemma goeswrong_silent_exclusive:
+  forall C st st' l l', mach_goes_wrong C st l -> mach_silent C st st' l' -> False.
+Proof.
+  intros C st st' l l' H H0.
+  destruct H as [pc [s_fin [H1 H2]]].
+  destruct H0 as [pc' [stk' [H1' H2']]].
+  eapply infseq_silent_finseq_excl.
+  eauto using machine_deterministic.
+  eauto. eapply H2. eauto. eauto using stop_irred.
+  destruct H2 as [A1 [A2 A3]].
+  eapply A2.
+Qed.
+
+Lemma goeswrong_reacts_exclusive:
+  forall C st l s, mach_goes_wrong C st l -> mach_reacts C st s -> False.
+Proof.
+  unfold mach_terminates, mach_reacts; intros.
+  destruct H as [pc [s_fin [H1 [H2 [H3 H4]]]]].
+  eapply infseq_finseq_excl.
+  eauto using machine_deterministic.
+  eauto. eapply H3.
+  eapply infseq_prod_infseq; eauto.
+Qed.
+
+Lemma goeswrong_OOM_exclusive:
+  forall C st l l', mach_goes_wrong C st l -> mach_OOM C st l' -> False.
+Proof.
+  unfold mach_goes_wrong, mach_OOM; intros.
+  destruct H as [pc [stk [st' [H2 [H3 H4]]]]].
+  assert ((Some (pc, stk, st') : configuration_limited) = (None : configuration_limited)).
+  { eapply finseq_unique; eauto using machine_deterministic, stop_irred.
+    unfold irred.  intros b l'' Hn. inversion Hn. }
+  congruence.
+Qed.
+
+Lemma terminates_silent_exclusive:
+  forall C st st' st'' l l', mach_terminates C st st' l -> mach_silent C st st'' l' -> False.
+Proof.
+  unfold mach_terminates, mach_silent; intros.
+  destruct H as [pc [H1 H2]].
+  destruct H0 as [pc' [stk' [H1' H2']]].
+  eapply infseq_silent_finseq_excl.
+  eauto using machine_deterministic.
+  eauto. eapply H2. eauto. eauto using stop_irred.
+Qed.
+
+(* Lemma silent_diverges_exclusive: *)
+(*   forall C st st' l s, mach_diverges C st s -> mach_silent C st st' l -> False. *)
+(* Proof. *)
+(*   unfold mach_diverges, mach_silent; intros. *)
+(*   destruct H0 as [pc [stk [H1 H2]]]. *)
+(*   (* eapply infseq_silent_excl. *) *)
+(*   eauto using machine_deterministic. *)
+(* Admitted. *)
+
+
+Lemma silent_reacts_exclusive:
+  forall C st st' s l,
+    mach_reacts C st s -> mach_silent C st st' l -> False.
+Proof.
+  intros C st st' s l H H0.
+  destruct H0 as [pc [stk [H0 H1]]].
+  (* inversion H; subst; clear H. *)
+  pose proof (star_infseq_prod_inv (machine_deterministic C) H0 H)
+    as [s' [H2 H3]].
+  inversion H2; subst; clear H2.
+  pose proof (infseq_silent_star_inv (machine_deterministic C) H4 H1).
+  destruct H2; now congruence.
+Qed.
+
+Lemma silent_OOM_exclusive:
+  forall C st st' l l', mach_OOM C st l -> mach_silent C st st' l' -> False.
+Proof.
+  unfold mach_terminates, mach_silent; intros.
+  (* destruct H as [pc [H1 H2]]. *)
+  destruct H0 as [pc' [stk' [H1' H2']]].
+  eapply infseq_silent_finseq_excl.
+  eauto using machine_deterministic.
+  eauto. eapply H. eauto. 
+  intros c l'' Hn; inversion Hn.
+Qed.
+
+Lemma reacts_OOM_exclusive:
+  forall C st s l,
+    mach_reacts C st s -> mach_OOM C st l -> False.
+Proof.
+  unfold mach_reacts, mach_OOM; intros.
+  eapply infseq_finseq_excl with (R := transition_limited C); eauto using machine_deterministic, stop_irred.
+  intros c l'' Hn; inversion Hn.
+  eapply infseq_prod_infseq.
+  eauto.
+Qed.
