ResourceExhaustion/Sequences.v
@@ -1,0 +1,609 @@
+(** A library of relation operators defining sequences of transitions
+  and useful properties about them. *)
+
+Set Implicit Arguments.
+
+Require Import Coq.Lists.List.
+Require Import Stream.
+Import ListNotations.
+
+Section Sequences_Traces.
+  Variable A E: Type.                 (**r the type of states *)
+  Variable R: A -> list E -> A -> Prop.       (**r the transition relation, from one state to the next *)
+
+  (** ** Finite sequences of transitions *)
+
+  (** Zero, one or several transitions: reflexive, transitive closure of [R]. *)
+  
+  Inductive star : A -> list E -> A -> Prop :=
+  | star_refl: forall a,
+      star a nil a
+  | star_step : forall a b c l1 l2,
+      R a l1 b -> star b l2 c -> star a (l1 ++ l2) c
+  .
+
+  Lemma star_one:
+    forall (a b: A) l, R a l b -> star a l b.
+  Proof.
+    intros a b l H.
+    replace l with (l ++ []); try now rewrite app_nil_r.
+    apply star_step with (b := b);
+      eauto using star.
+  Qed.
+
+  Lemma starans:
+    forall (a b: A) (lab : list E), star a lab b ->
+                               forall c (lbc : list E), star b lbc c -> star a (lab ++ lbc) c.
+  Proof.
+    intros a b lab Hab.
+    induction Hab; intros.
+    assumption.
+    rewrite <- app_assoc.
+    eapply star_step. eassumption.
+    apply IHHab. eassumption.
+  Qed.
+
+  (** One or several transitions: transitive closure of [R]. *)
+
+  Inductive plus: A -> list E -> A -> Prop :=
+  | plus_left : forall a b c l l',
+      R a l b -> star b l' c -> plus a (l ++ l') c.
+
+  Lemma plus_one:
+    forall a b l, R a l b -> plus a l b.
+  Proof.
+    intros a b l H.
+    replace l with (l ++ []);
+      eauto using star, plus.
+    now rewrite app_nil_r.
+  Qed.
+
+  Lemma plus_star:
+    forall a b l,
+      plus a l b -> star a l b.
+  Proof.
+    intros. inversion H; eauto using star.
+  Qed.
+
+  Lemma plus_starans:
+    forall a b c lab lbc, plus a lab b -> star b lbc c ->
+                     plus a (lab ++ lbc) c.
+  Proof.
+    intros. inversion H; subst; eauto using plus, starans.
+    rewrite <- app_assoc.
+    eapply plus_left. eassumption.
+    eapply starans; eauto.
+  Qed.
+
+  Lemma star_plusans:
+    forall a b c lab lbc, star a lab b -> plus b lbc c ->
+                     plus a (lab ++ lbc) c.
+  Proof.
+    intros.
+    inversion H0; inversion H; subst;
+      eauto using plus_left, plus, star, starans.
+    rewrite <- app_assoc.
+    eapply plus_left; eauto using star, starans.
+  Qed.
+
+  Lemma plus_right:
+    forall a b c l l', star a l b -> R b l' c -> plus a (l ++ l') c.
+  Proof.
+    intros a b c l  l' H H0.
+    eapply star_plusans. eauto. apply plus_one; eauto.
+  Qed.
+
+  (** ** Infinite sequences of transitions *)
+
+  Variable measure: A -> nat.                  (**r the anti-stuttering measure *)
+
+  (* Infinite execution: either produces the whole stream, or a prefix and then
+     silent divergence *)
+  CoInductive infseq: @stream E -> A -> Prop :=
+  | infseq_step: forall a s b l,
+      R a l b -> infseq s b -> infseq (Stream.app_list_stream l s) a.
+
+  (* CF CompCert smallstep file *)
+  CoInductive infseq_N : @stream E -> nat -> A -> Prop :=
+  | infseq_N_star : forall a b n1 n2 l s,
+      n2 < n1 ->
+      star a l b ->
+      infseq_N s n2 b ->
+      infseq_N (Stream.app_list_stream l s) n1 a
+  | infseq_N_plus : forall a b n1 n2 l s,
+      plus a l b ->
+      infseq_N s n2 b ->
+      infseq_N (Stream.app_list_stream l s) n1 a.
+
+  Lemma infseq_N_inv : forall n s a,
+      infseq_N s n a ->
+      exists l, exists s', exists n', exists a',
+              R a l a' /\ infseq_N s' n' a' /\ Stream.app_list_stream l s' = s.
+  Proof.
+    intros n. pattern n.
+    eapply well_founded_ind with (R := lt).
+    apply PeanoNat.Nat.lt_wf_0.
+    intros x H s a H0.
+    inversion H0; subst; clear H0.
+    - inversion H2; subst; clear H2.
+      + apply H with n2. now apply H1.
+        apply H3.
+      + exists l1. exists (app_list_stream l2 s0). exists x. exists b0.
+        repeat split; eauto.
+        eapply infseq_N_star; eauto.
+        clear.
+        induction l1; eauto.
+        simpl; now rewrite IHl1.
+    - inversion H1; subst; clear H1.
+      exists l0, (app_list_stream l' s0), n2, b0.
+      repeat split; eauto.
+      inversion H3; subst; clear H3.
+      assumption.
+      eapply infseq_N_plus; eauto.
+      econstructor; eauto.
+      clear.
+      induction l0; eauto.
+      simpl; now rewrite IHl0.
+  Qed.
+
+  Lemma infseq_N_infseq :
+    forall a s n, infseq_N s n a -> infseq s a.
+  Proof.
+    cofix Hfix.
+    intros a s n H.
+    destruct (infseq_N_inv H) as [l [s' [n' [a' [HR [Hinf Heq]]]]]].
+    subst.
+    apply infseq_step with (b := a').
+    eauto.
+    eapply Hfix; eauto.
+  Qed.
+
+  Lemma infseq_infseq_N :
+    forall a n s, infseq s a -> infseq_N s n a.
+  Proof.
+    cofix Hfix.
+    intros a n s H.
+    inversion H; subst.
+    eapply infseq_N_plus with (n2 := 0).
+    replace l with (l ++ []) by now rewrite app_nil_r.
+    econstructor. eauto. econstructor.
+    eapply Hfix. eauto.
+  Qed.
+
+  (* Now, we can start defining interesting notions of infseq.
+     [infseq_prod s a] means that [a] actually produces the stream [s]*)
+  CoInductive infseq_prod : @stream E -> A -> Prop :=
+  | infseq_prod_star: forall a b l s,
+      star a l b ->
+      l <> [] ->
+      infseq_prod s b ->
+      infseq_prod (app_list_stream l s) a
+  .
+
+  Lemma star_infseq_prod : forall a b l s,
+      star a l b ->
+      infseq_prod s b ->
+      infseq_prod (app_list_stream l s) a.
+  Proof.
+    intros a b l s H H0.
+    inversion H0; subst.
+    assert (star a (l ++ l0) b0) by now eapply starans; eauto.
+    replace (app_list_stream l (app_list_stream l0 s0)) with (app_list_stream (l ++ l0) s0).
+    econstructor; eauto.
+    now destruct l, l0.
+    clear.
+    induction l; auto.
+    now simpl; rewrite IHl.
+  Qed.
+
+  Lemma star_inv : forall a l b,
+      star a l b ->
+      (a = b /\ l = []) \/ plus a l b.
+  Proof.
+    intros a l b H.
+    inversion H; subst; clear H.
+    - left; auto.
+    - right; econstructor; eauto.
+  Qed.
+
+  Lemma star_infseq : forall a l b s,
+      star a l b ->
+      infseq s b ->
+      infseq (app_list_stream l s) a.
+  Proof.
+    intros a l b s H H0.
+    induction H.
+    - eauto.
+    - rewrite app_list_stream_app.
+      now econstructor; eauto.
+  Qed.
+
+  Lemma infseq_prod_infseq : forall s a,
+      infseq_prod s a ->
+      infseq s a.
+  Proof.
+    assert (forall s a n, infseq_prod s a -> infseq_N s n a).
+    {
+      cofix Hfix.
+      intros s a n H.
+      inversion H; subst.
+      destruct l as [| e l]; try congruence.
+      replace (app_list_stream (e :: l) s0) with (app_list_stream ([e] ++ l) s0) in H by reflexivity.
+      destruct (star_inv H0) as [[] |]; try congruence.
+      inversion H3; subst; clear H3.
+      rewrite app_list_stream_app.
+      eapply infseq_N_plus.
+      - eapply plus_one. eauto.
+      - eapply Hfix.
+        replace ([e] ++ l) with (e :: l) in H by reflexivity.
+        rewrite <- H4 in H.
+        eapply star_infseq_prod.
+        eauto. eauto.
+    }
+    intros s a H0.
+    eapply infseq_N_infseq.
+    eapply H.
+    eassumption.
+    Unshelve.
+    all: exact 0.
+  Qed.
+
+  (* Infinitely many silent steps *)
+  CoInductive infseq_silent: A -> Prop :=
+  | infseq_silent_step: forall a b,
+      R a [] b -> infseq_silent b -> infseq_silent a.
+
+  (* CF CompCert smallstep file *)
+  CoInductive infseq_silent_N : nat -> A -> Prop :=
+  | infseq_silent_N_star : forall a b n1 n2 ,
+      n2 < n1 ->
+      star a [] b ->
+      infseq_silent_N n2 b ->
+      infseq_silent_N n1 a
+  | infseq_silent_N_plus : forall a b n1 n2,
+      plus a [] b ->
+      infseq_silent_N n2 b ->
+      infseq_silent_N n1 a.
+
+  Lemma infseq_silent_N_inv : forall n a,
+      infseq_silent_N n a ->
+      exists n', exists a',
+          R a [] a' /\ infseq_silent_N n' a'. 
+  Proof.
+    intros n. pattern n.
+    eapply well_founded_ind with (R := lt).
+    apply PeanoNat.Nat.lt_wf_0.
+    intros x H a H0.
+    inversion H0; subst; clear H0.
+    - inversion H2; subst; clear H2.
+      + apply H with n2. now apply H1.
+        apply H3.
+      + exists x. exists b0.
+        assert (Heq: l1 = [] /\ l2 = []) by now apply app_eq_nil.
+        destruct Heq; subst.
+        split; auto.
+        eapply infseq_silent_N_star; eauto.
+    - inversion H1; subst; clear H1.
+      exists n2, b0.
+      assert (Heq: l = [] /\ l' = []) by now apply app_eq_nil.
+      destruct Heq; subst.
+      split; auto.
+      inversion H5; subst; clear H5.
+      assumption.
+      eapply infseq_silent_N_plus; eauto.
+      rewrite <- H1.
+      econstructor; eauto.
+  Qed.
+
+  Lemma infseq_silent_N_infseq_silent :
+    forall a n, infseq_silent_N n a -> infseq_silent a.
+  Proof.
+    cofix Hfix.
+    intros a n H.
+    destruct (infseq_silent_N_inv H) as [n' [a' [Hr Hinf]]].
+    apply infseq_silent_step with (b := a').
+    eauto.
+    eapply Hfix; eauto.
+  Qed.
+
+  Lemma infseq_silent_infseq_silent_N :
+    forall a n, infseq_silent a -> infseq_silent_N n a.
+  Proof.
+    cofix Hfix.
+    intros a n H.
+    inversion H; subst.
+    eapply infseq_silent_N_plus with (n2 := 0).
+    replace [] with ([] ++ [] : list E) by reflexivity.
+    econstructor; eauto; eapply star_refl.
+    now eapply Hfix.
+  Qed.
+
+  Lemma infseq_silent_infseq :
+    forall a s, infseq_silent a -> infseq s a.
+  Proof.
+    cofix Hfix.
+    intros a s H.
+    inversion H; subst; clear H.
+    replace s with (app_list_stream [] s) by reflexivity.
+    econstructor; eauto.
+  Qed.
+
+  Lemma infseq_infseq_silent :
+    forall P s a, (infseq s a -> P a) ->
+             (infseq_silent a -> P a).
+  Proof.
+    intros P s a X H.
+    apply X. now apply infseq_silent_infseq.
+  Qed.
+
+
+  Lemma diverges_infseq_silent:
+    forall s0,
+      (forall s1 t1, star s0 t1 s1 -> exists s2, R s1 [] s2) ->
+      infseq_silent s0.
+  Proof.
+    cofix Hfix; intros.
+    destruct (H s0 []) as [s1 H']. constructor.
+    econstructor; try eassumption.
+    apply Hfix.
+    intros s2 t1 H0.
+    eapply H. eapply star_step; eauto.
+  Qed.
+
+  Definition irred (a: A) : Prop := forall b e, ~(R a e b).
+
+  (* Inductive behavior := *)
+  (* | Reactive : @stream E -> behavior *)
+  (* | Diverges : list E -> behavior *)
+  (* | Terminates : list E -> behavior *)
+  (* . *)
+
+  (** ** Determinism properties for functional transition relations. *)
+
+  (** A transition relation is functional if every state can transition to at most
+  one other state. *)
+
+  Hypothesis R_functional:
+    forall a b c l1 l2, R a l1 b -> R a l2 c -> b = c /\ l1 = l2.
+
+  Lemma star_infseq_prod_inv : forall a l b,
+      star a l b ->
+      forall s, infseq_prod s a ->
+           exists s', infseq_prod s' b /\ s = app_list_stream l s'.
+  Proof.
+    induction 1; intros.
+    - eexists; eauto.
+    - inversion H1; subst; clear H1.
+      inversion H2; subst; clear H2.
+      congruence.
+      assert (b1 = b /\ l0 = l1) as [? ?]
+          by (now eapply R_functional; eassumption); subst.
+      specialize (IHstar (app_list_stream l3 s0)).
+      destruct IHstar as [s' [? ?]].
+      eapply star_infseq_prod; eauto.
+      exists s'. split; eauto.
+      clear -H6.
+      induction l1. simpl. rewrite H6. reflexivity.
+      simpl. rewrite IHl1. reflexivity.
+  Qed.
+
+
+  Lemma infseq_prod_inv : forall a l1 b,
+      star a l1 b ->
+      forall c l2 s1 s2,
+        star a l2 c ->
+        l1 <> [] -> l2 <> [] ->
+        infseq_prod s1 b ->
+        infseq_prod s2 c ->
+        exists a', exists l, exists s1', exists s2',
+                l <> [] /\
+                infseq_prod s1' a' /\ infseq_prod s2' a' /\
+                app_list_stream l1 s1 = app_list_stream l s1' /\
+                app_list_stream l2 s2 = app_list_stream l s2'.
+  Proof.
+    induction 1; intros.
+    congruence.
+    inversion H1; subst; clear H1. congruence.
+    assert (b = b0 /\ l1 = l3) as [? ?] by (eapply R_functional; eassumption); subst.
+    destruct l3.
+    - simpl in *. eapply IHstar; eauto.
+    - exists b0. exists (e :: l3). exists (app_list_stream l2 s1). exists (app_list_stream l4 s2).
+      repeat split.
+      congruence.
+      eapply star_infseq_prod; eauto.
+      eapply star_infseq_prod; eauto.
+      eapply app_list_stream_app. eapply app_list_stream_app.
+  Qed.
+
+
+  (** Uniqueness of finite transition sequences. *)
+
+  Lemma star_star_inv:
+    forall a b l1, star a l1 b ->
+              forall c l2, star a l2 c ->
+                      (exists l3, l1 = l2 ++ l3 /\ star c l3 b) \/
+                      (exists l3, l2 = l1 ++ l3 /\ star b l3 c).
+  Proof.
+    induction 1; intros.
+    - right; now eexists.
+    - inversion H1; subst.
+      + left. eexists; split; eauto using star.
+        now rewrite app_nil_l.
+      + assert (b = b0) by (eapply R_functional; eauto).
+        assert (He: l1 = l3) by (eapply R_functional; eauto).
+        subst b0 l3.
+        edestruct (IHstar c0) as [[l3 [IH1 IH2]] | [l3 [IH1 IH2]]]. eauto.
+        * subst.
+          left.
+          eexists; split; eauto using star.
+          now rewrite app_assoc.
+        * subst.
+          right.
+          eexists; split; eauto using star.
+          now rewrite app_assoc.
+  Qed.
+
+  Lemma finseq_unique:
+    forall a b b' l l',
+      star a l b -> irred b ->
+      star a l' b' -> irred b' ->
+      b = b' /\ l = l'.
+  Proof.
+    intros.
+    destruct (star_star_inv H H1) as [[l'' [H3 H4]] | [l'' [H3 H4]]].
+    - inversion H4; split; subst; auto; try elim (H2 _ _ H5).
+      apply app_nil_r.
+    - inversion H4; split; subst; auto; try elim (H0 _ _ H5).
+      now rewrite app_nil_r.
+  Qed.
+
+  Lemma infseq_silent_star_inv : forall a b l,
+    star a l b ->
+    infseq_silent a ->
+    l = [] /\ infseq_silent b.
+  Proof.
+    intros a b l H.
+    induction H.
+    - auto.
+    - intros H1.
+      inversion H1; subst; clear H1.
+      destruct (R_functional H H2); subst; eauto.
+  Qed.
+   
+
+
+  (** A state cannot both diverge and terminate on an irreducible state. *)
+
+  (* Lemma infseq_star_inv: *)
+  (*   forall a b l s, star a l b -> infseq s a -> infseq (l++s) b. *)
+  (* Proof. *)
+  (*   induction 1; intros. *)
+  (* - auto. *)
+  (* - inversion H1; subst. *)
+  (*   assert (b = b0) by (eapply R_functional; eauto). subst b0. *)
+  (*   apply IHstar; auto. *)
+  (* Qed. *)
+
+  Lemma infseq_finseq_excl:
+    forall a b l s,
+      star a l b -> irred b -> infseq s a -> False.
+  Proof.
+    intros.
+    assert (exists s', infseq s' b).
+    { generalize dependent s.
+      induction H; intros.
+      - inversion H1; subst; elim (H0 _ _ H).
+      - inversion H2; subst.
+        + assert (b = b0) by (eapply R_functional; eauto).
+          subst b0.
+          eapply IHstar; eassumption.
+    }
+    destruct H2 as [s' Hs'].
+    inversion Hs'; subst; elim (H0 _ _ H2).
+  Qed.
+
+  Lemma infseq_silent_irred_excl:
+    forall a,
+      irred a -> infseq_silent a -> False.
+  Proof.
+    intros a H H0.
+    unfold irred in *.
+    destruct H0.
+    now apply (H b []).
+  Qed.
+
+  Lemma infseq_silent_finseq_excl:
+    forall a b c l l',
+      star a l b ->
+      star a l' c ->
+      infseq_silent b ->
+      irred c ->
+      False.
+  Proof.
+    intros a b c l l' H H0 H1 H2.
+    destruct (star_star_inv H H0) as [[l'' [H3 H4]] | [l'' [H3 H4]]].
+    - inversion H4; subst.
+      + now eapply infseq_silent_irred_excl.
+      + unfold irred in H2.
+        eapply H2; eassumption.
+    - induction H4; subst.
+      + now eapply infseq_silent_irred_excl.
+      + inversion H1; subst.
+        assert (b = b0 /\ l1 = []) as [? ?] by (eapply R_functional; eauto); subst.
+        simpl in *.
+        apply IHstar; eauto.
+        replace l with (l ++ []) by now apply app_nil_r.
+        eapply starans. eauto.
+        replace [] with ([] ++ [] : list E) by reflexivity.
+        econstructor; eauto. constructor.
+  Qed.
+
+  (** If there exists an infinite sequence of transitions from [a],
+  all sequences of transitions arising from [a] are infinite. *)
+
+  (* Lemma infseq_all_seq_inf: *)
+  (*   forall a, infseq a -> all_seq_inf a. *)
+  (* Proof. *)
+  (*   intros. unfold all_seq_inf. intros.  *)
+  (*   assert (infseq b) by (eapply infseq_star_inv; eauto).  *)
+  (*   inversion H1. subst. exists b0; auto. *)
+  (* Qed. *)
+
+  Lemma plus_infseq :
+    forall a b s l,
+      plus a l b -> infseq s b ->
+      infseq (Stream.app_list_stream l s) a.
+  Proof.
+    intros until l.
+    intros H.
+    inversion H; subst.
+    eapply star_infseq.
+    econstructor; eauto.
+  Defined.
+
+  (** Alternative view of streams *)
+  CoInductive stream' :=
+  | scons' : forall (l : list E) (s : stream'), l <> [] -> stream'.
+
+  Program Definition split_traceinf' (l : list E) (s: stream') (NE: l <> []): E * stream' :=
+    match l with
+    | nil => _
+    | e :: nil => (e, s)
+    | e :: t' => (e, @scons' t' s _)
+    end.
+  Next Obligation.
+    destruct t'; congruence.
+  Qed.
+
+  CoFixpoint stream_of_stream' (s': stream') : stream :=
+    match s' with
+    | @scons' t T'' NOTEMPTY =>
+      let (e, tl) := @split_traceinf' t T'' NOTEMPTY in
+      scons e (stream_of_stream' tl)
+    end.
+
+  Remark unroll_stream':
+    forall T, T = match T with @scons' t T' NE => @scons' t T' NE end.
+  Proof.
+    intros. destruct T; auto.
+  Qed.
+
+  Remark unroll_stream:
+    forall (T : @stream E), T = match T with scons t T' => scons t T' end.
+  Proof.
+    intros. destruct T; auto.
+  Qed.
+
+  Lemma stream_stream'_app:
+    forall t T NE,
+      stream_of_stream' (@scons' t T NE) = Stream.app_list_stream t (stream_of_stream' T).
+  Proof.
+    induction t.
+    intros. elim NE. auto.
+    intros. simpl.
+    rewrite (unroll_stream (stream_of_stream' (@scons' (a :: t) T NE))).
+    simpl. destruct t. auto.
+    simpl. f_equal. apply IHt.
+  Qed.
+
+End Sequences_Traces.
