Robust2relSSCHCriterion.v
@@ -1,0 +1,153 @@
+From mathcomp Require Import all_ssreflect.
+
+Set Implicit Arguments.
+Unset Printing Implicit Defensive.
+
+Require Import ClassicalExtras.
+Require Import MyNotation.
+Require Import Setoid.
+Require Import FunctionalExtensionality.
+
+Require Import Galois.
+Require Import LanguageModel.
+Require Import TraceModel.
+Require Import Properties.
+Require Import ChainModel.
+Require Import Robust2relSSCHPreservation.
+
+Require Import PropExtensionality.
+Definition prop_extensionality := propositional_extensionality.
+
+Section Robust2relCrit.
+
+  Variable Source Target: Language.
+  Variable compilation_chain : CompilationChain Source Target.
+
+  (*CA: we don't need a particular structure of traces to define preservation
+        e.g. traces = values or our defn of traces both make sense
+   *)
+  Variable trace__S trace__T : Type.
+
+  Local Definition prop__S := prop trace__S.
+  Local Definition prop__T := prop trace__T.
+
+  Variable Source_Semantics : Semantics Source trace__S.
+  Variable Target_Semantics : Semantics Target trace__T.
+
+  Local Definition sem__S := sem Source_Semantics.
+  Local Definition sem__T := sem Target_Semantics.
+  Local Definition beh__S := beh Source_Semantics.
+  Local Definition beh__T := beh Target_Semantics.
+  Local Definition par__S := par Source.
+  Local Definition par__T := par Target.
+  Local Definition ctx__S := ctx Source.
+  Local Definition ctx__T := ctx Target.
+  Local Definition rhsat__S := rhsat2 Source_Semantics.
+  Local Definition rhsat__T := rhsat2 Target_Semantics.
+
+  Local Definition cmp := compile_par Source Target compilation_chain.
+
+  Local Notation "P ↓" := (cmp P) (at level 50).
+ (* CA: don't understand why this does not work
+
+   Local Notation " C [ P ] " := (plug _  P C) (at level 50).
+  *)
+  Local Definition plug__S:= plug Source.
+  Local Definition plug__T := plug Target.
+
+  Variable rel : trace__S -> trace__T -> Prop.
+
+  (* __π to highlights these maps are mappings between properties  *)
+  Local Definition σ__π : (trace__T -> Prop) -> (trace__S -> Prop) :=
+                       γ (@induced_connection (trace__T) (trace__S) rel).
+
+  Local Definition τ__π : (trace__S -> Prop) -> (trace__T -> Prop) :=
+                       α (@induced_connection (trace__T) (trace__S) rel).
+
+  Local Definition induced_adj : Adjunction_law τ__π σ__π :=
+    adjunction_law (induced_connection rel).
+
+  Lemma τ__π_mono : monotone τ__π.
+  Proof. move: induced_adj. rewrite Galois_equiv. easy. Qed.
+
+  Local Definition σ : (prop__T * prop__T -> Prop) -> (prop__S * prop__S -> Prop) := prod_σ σ__π.
+  Local Definition τ : (prop__S * prop__S -> Prop) -> (prop__T * prop__T -> Prop) := prod_τ τ__π.
+
+
+  Local Definition sCl_σR2rhP := sCl_σR2rhP compilation_chain
+                                           Source_Semantics Target_Semantics
+                                           σ__π.
+
+  Local Definition sCl_τR2rhP := sCl_τR2rhP compilation_chain
+                                        Source_Semantics Target_Semantics
+                                        τ__π.
+
+  Definition rel_R2rSCHC : Prop :=
+    forall C__T P1 P2, exists C__S,
+        forall t1 t2, sem__T (plug__T (P1 ↓) C__T) t1 ->
+                  sem__T (plug__T (P2 ↓) C__T) t2 ->
+           exists s1 s2, rel s1 t1 /\
+                     rel s2 t2 /\
+                     sem__S (plug__S P1 C__S) s1 /\
+                     sem__S (plug__S P2 C__S) s2.
+
+  Lemma rel_R2rSCHC_conclusion (C__T : ctx__T) (P1 P2 : par__S) (C__S : ctx__S):
+    (forall t1 t2, sem__T (plug__T (P1 ↓) C__T) t1 ->
+               sem__T (plug__T (P2 ↓) C__T) t2 ->
+           exists s1 s2, rel s1 t1 /\
+                     rel s2 t2 /\
+                     sem__S (plug__S P1 C__S) s1 /\
+                     sem__S (plug__S P2 C__S) s2 ) <->
+    (beh__T (plug__T (P1 ↓) C__T)) ⊆ τ__π (beh__S (plug__S P1 C__S)) /\
+    (beh__T (plug__T (P2 ↓) C__T)) ⊆ τ__π (beh__S (plug__S P2 C__S)).
+  Proof.
+    split.
+    + move => lhs. split.
+         move => t1 Hsem1. destruct (non_empty_sem Target_Semantics (plug__T (P2 ↓) C__T)) as [t2 Hsem2].
+         destruct (lhs t1 t2 Hsem1 Hsem2) as [s1 [s2 [rel1 [rel2 [Hsem1' Hsem2']]]]].
+         now exists s1.
+       move => t2 Hsem2. destruct (non_empty_sem Target_Semantics (plug__T (P1 ↓) C__T)) as [t1 Hsem1].
+       destruct (lhs t1 t2 Hsem1 Hsem2) as [s1 [s2 [rel1 [rel2 [Hsem1' Hsem2']]]]].
+       now exists s2.
+    + move => [H1 H2] t1 t2 Hsem1 Hsem2.
+      move: (H1 t1 Hsem1) (H2 t2 Hsem2). rewrite /τ__π /α /induced_connection /low_rel /=.
+        by firstorder.
+   Qed.
+
+  Theorem rel_R2rSCHC_sCl_τR2rSCHP :
+    rel_R2rSCHC <->
+    (forall (P1 P2 : par__S) S, SCH2 S -> sCl_τR2rhP P1 P2 S).
+  Proof.
+    split.
+    - move => Htilde P1 P2 S S_ssc. setoid_rewrite contra_τR2rhP.
+      move => [C__T Hsem].
+      move: (Htilde C__T P1 P2) => [C__S HH].
+      exists C__S => Hfalse.
+      apply: Hsem.
+      exists (τ__π (beh__S (plug__S P1 C__S))), (τ__π (beh__S (plug__S P2 C__S))). split.
+      + by exists (beh__S (plug__S P1 C__S)), (beh__S (plug__S P2 C__S)).
+      + by rewrite //= -rel_R2rSCHC_conclusion.
+    - move => Hτ C__T P1 P2.
+      have Hssc : SCH2 (fun b: prop__S * prop__S =>  ~ (beh__T (plug__T (P1 ↓) C__T) ⊆ τ__π (fst b) /\
+                                                  beh__T (plug__T (P2 ↓) C__T) ⊆ τ__π (snd b))).
+      { rewrite /SCH2. move => β1 β2 β1' β2' Hb  b1_b1 b2_b2 [Hf1 Hf2].
+        apply: Hb. split;
+        apply: subset_trans; eauto; rewrite /=; by apply: τ__π_mono. }
+      specialize (Hτ P1 P2 _ Hssc).
+      apply contra in Hτ. move: Hτ. rewrite !neg_rhsat2 /=.
+      move => [Cs Hbeh]. exists Cs.
+      rewrite rel_R2rSCHC_conclusion. by move/NNPP: Hbeh.
+      rewrite neg_rhsat2. exists C__T. move => [b1[ b2 Hf]].
+      move: Hf. rewrite /prod_τ /=. move => [[π__S [π__S' [Heq1 [Heq2 Hn]]]] [H1 H2]].
+      subst. by apply: Hn.
+  Qed.
+
+  Theorem rel_R2rTC_σR2rTP :
+    rel_R2rSCHC <->
+    (forall (P1 P2 : par__S) T, SCH2 T -> sCl_σR2rhP P1 P2 T).
+  Proof.
+    setoid_rewrite  (Adj_sCl_σR2rSCHP_iff_sCl_τR2rSCHP _ _ _ induced_adj).
+    by rewrite rel_R2rSCHC_sCl_τR2rSCHP.
+  Qed.
+
+End Robust2relCrit.
