Robust2relTraceCriterion.v
@@ -1,0 +1,110 @@
+From mathcomp Require Import all_ssreflect.
+
+Set Implicit Arguments.
+Unset Printing Implicit Defensive.
+
+Require Import ClassicalExtras.
+Require Import MyNotation.
+Require Import Setoid.
+Require Import FunctionalExtensionality.
+
+Require Import Galois.
+Require Import LanguageModel.
+Require Import TraceModel.
+Require Import Properties.
+Require Import ChainModel.
+Require Import Robust2relTraceProperty.
+
+Require Import PropExtensionality.
+Definition prop_extensionality := propositional_extensionality.
+
+Section Robust2relCrit.
+
+  Variable Source Target: Language.
+  Variable compilation_chain : CompilationChain Source Target.
+
+  (*CA: we don't need a particular structure of traces to define preservation
+        e.g. traces = values or our defn of traces both make sense
+   *)
+  Variable trace__S trace__T : Set.
+
+  Local Definition prop__S := prop trace__S.
+  Local Definition prop__T := prop trace__T.
+
+  Variable Source_Semantics : Semantics Source trace__S.
+  Variable Target_Semantics : Semantics Target trace__T.
+
+  Local Definition sem__S := sem Source_Semantics.
+  Local Definition sem__T := sem Target_Semantics.
+  Local Definition par__S := par Source.
+  Local Definition par__T := par Target.
+  Local Definition ctx__S := ctx Source.
+  Local Definition ctx__T := ctx Target.
+  Local Definition rsat__S := rsat2 Source_Semantics.
+  Local Definition rsat__T := rsat2 Target_Semantics.
+
+  Local Definition cmp := compile_par Source Target compilation_chain.
+
+  Local Notation "P ↓" := (cmp P) (at level 50).
+ (* CA: don't understand why this does not work
+
+   Local Notation " C [ P ] " := (plug _  P C) (at level 50).
+  *)
+  Local Definition plug__S:= plug Source.
+  Local Definition plug__T := plug Target.
+
+  Variable rel : trace__S -> trace__T -> Prop.
+
+  Local Definition σ : (trace__T * trace__T -> Prop) -> (trace__S * trace__S -> Prop) :=
+                       γ (@induced_connection_prod (trace__T) (trace__S) rel).
+
+  Local Definition τ : (trace__S * trace__S -> Prop) -> (trace__T * trace__T -> Prop) :=
+                       α (@induced_connection_prod (trace__T) (trace__S) rel).
+
+
+  Local Definition σR2rTP := σR2rTP compilation_chain
+                                    Source_Semantics Target_Semantics
+                                    σ.
+
+  Local Definition τR2rTP := τR2rTP compilation_chain
+                                    Source_Semantics Target_Semantics
+                                    τ.
+
+
+  Local Definition induced_adj : Adjunction_law τ σ :=
+    adjunction_law (induced_connection_prod rel).
+
+  Definition rel_R2rTC : Prop :=
+    forall C__T P1 P2 t1 t2, sem__T (plug__T (P1 ↓) C__T) t1 ->
+                       sem__T (plug__T (P2 ↓) C__T) t2 ->
+                       exists C__S s1 s2, rel s1 t1 /\
+                                    rel s2 t2 /\
+                                    sem__S (plug__S P1 C__S) s1 /\
+                                    sem__S (plug__S P2 C__S) s2.
+
+  Theorem rel_R2rTC_τR2rTP : rel_R2rTC <-> τR2rTP.
+  Proof.
+    setoid_rewrite contra_τR2rTP. split.
+    + move => Hrel P1 P2 S [C__T [t1 [t2 [Hsem1 [Hsem2 τS_t1_t2]]]]].
+      destruct (Hrel C__T P1 P2 t1 t2 Hsem1 Hsem2) as
+          [C__S [s1 [s2 [rel1 [rel2 [Hsem1' Hsem2' ]]]]]].
+      exists C__S, s1, s2. repeat (split; auto).
+      move => HS_s1_s2.
+      apply: τS_t1_t2. exists (s1, s2). repeat (split; auto).
+    + move => Hτ C__T P1 P2 t1 t2 Hsem1 Hsem2.
+      specialize (Hτ P1 P2 (fun s => ~ rel (fst s) t1 \/ ~ rel (snd s) t2)).
+      destruct Hτ as [C__S [s1 [s2 [Hsem1' [Hsem2' notS_s1_s2]]]]].
+      ++ exists C__T, t1, t2. repeat (split; auto).
+         move => [[s1 s2] [Hs1_s2 [H1 H2]]].
+         destruct Hs1_s2; contradiction.
+      move/de_morgan1: notS_s1_s2. rewrite -dne. move => [rel1 rel2].
+      exists C__S, s1, s2. repeat (split; auto).
+  Qed.
+
+  Theorem rel_R2rTC_σR2rTP : rel_R2rTC <-> σR2rTP.
+  Proof.
+    setoid_rewrite (Adj_σR2rTP_iff_τR2rTP _ _ _ induced_adj).
+    by rewrite rel_R2rTC_τR2rTP.
+  Qed.
+
+End Robust2relCrit.
