Robust2relTraceProperty.v
@@ -1,0 +1,131 @@
+From mathcomp Require Import all_ssreflect.
+
+Set Implicit Arguments.
+Unset Printing Implicit Defensive.
+
+Require Import ClassicalExtras.
+Require Import MyNotation.
+Require Import Setoid.
+Require Import FunctionalExtensionality.
+
+Require Import Galois.
+Require Import LanguageModel.
+Require Import TraceModel.
+Require Import Properties.
+Require Import ChainModel.
+
+Require Import PropExtensionality.
+Definition prop_extensionality := propositional_extensionality.
+
+Section Robust2relPreservation.
+
+  Variable Source Target: Language.
+  Variable compilation_chain : CompilationChain Source Target.
+
+  (*CA: we don't need a particular structure of traces to define preservation
+        e.g. traces = values or our defn of traces both make sense
+   *)
+  Variable trace__S trace__T : Set.
+
+  Local Definition prop__S := prop trace__S.
+  Local Definition prop__T := prop trace__T.
+
+  Variable Source_Semantics : Semantics Source trace__S.
+  Variable Target_Semantics : Semantics Target trace__T.
+
+  Local Definition sem__S := sem Source_Semantics.
+  Local Definition sem__T := sem Target_Semantics.
+  Local Definition par__S := par Source.
+  Local Definition par__T := par Target.
+  Local Definition ctx__S := ctx Source.
+  Local Definition ctx__T := ctx Target.
+  Local Definition rsat__S := rsat2 Source_Semantics.
+  Local Definition rsat__T := rsat2 Target_Semantics.
+
+  Local Definition cmp := compile_par Source Target compilation_chain.
+
+  Local Notation "P ↓" := (cmp P) (at level 50).
+ (* CA: don't understand why this does not work
+
+   Local Notation " C [ P ] " := (plug _  P C) (at level 50).
+  *)
+  Local Definition plug__S:= plug Source.
+  Local Definition plug__T := plug Target.
+
+  Variable σ : (trace__T * trace__T -> Prop) -> (trace__S * trace__S -> Prop).
+  Variable τ : (trace__S * trace__S -> Prop) -> (trace__T * trace__T -> Prop).
+
+  Definition σR2rP (P1 P2 : par__S) (T : trace__T * trace__T -> Prop) :=
+    rsat__S P1 P2 (σ T) -> rsat__T (P1 ↓) (P2 ↓) T.
+
+  Definition σR2rTP := forall P1 P2 T, σR2rP P1 P2 T.
+
+  Lemma contra_σR2rP (P1 P2 : par__S) (T : trace__T * trace__T -> Prop) :
+    (σR2rP P1 P2 T) <->  ((exists C__T t1 t2, sem__T ( plug__T (P1 ↓) C__T) t1 /\
+                                      sem__T ( plug__T (P2 ↓) C__T) t2 /\  ~ (T (t1,t2))) ->
+                        (exists C__S s1 s2, sem__S (plug__S P1 C__S) s1 /\
+                                      sem__S (plug__S P2 C__S) s2 /\
+                                    ~ (σ T) (s1, s2))).
+  Proof.
+    rewrite /σR2rP. by rewrite [_ -> _] contra !neg_rsat2.
+  Qed.
+
+  Lemma contra_σR2rTP :
+    σR2rTP <-> (forall P1 P2 T, (exists C__T t1 t2, sem__T (plug__T (P1 ↓) C__T) t1 /\
+                                       sem__T (plug__T (P2 ↓) C__T) t2 /\
+                                     ~ (T (t1, t2))) ->
+                        (exists C__S s1 s2, sem__S (plug__S P1 C__S) s1 /\
+                                      sem__S (plug__S P2 C__S) s2 /\
+                                     ~ (σ T) (s1, s2))).
+  Proof.
+    rewrite /σR2rTP.
+    split => H P1 P2 T; by move/contra_σR2rP: (H P1 P2 T).
+  Qed.
+
+  Definition τR2rP (P1 P2 : par__S) (S : trace__S * trace__S -> Prop) :=
+    rsat__S P1 P2 S -> rsat__T (P1 ↓) (P2 ↓) (τ S).
+
+  Definition τR2rTP := forall P1 P2 S, τR2rP P1 P2 S.
+
+  Lemma contra_τR2rP (P1 P2 : par__S) (S : trace__S * trace__S -> Prop) :
+    (τR2rP P1 P2 S) <-> ((exists C__T t1 t2, sem__T (plug__T (P1 ↓) C__T) t1 /\
+                                    sem__T (plug__T (P2 ↓) C__T) t2 /\
+                                   ~ (τ S) (t1, t2)) ->
+                      (exists C__S s1 s2, sem__S (plug__S P1 C__S) s1 /\
+                                    sem__S (plug__S P2 C__S) s2 /\
+                                   ~ S (s1, s2))).
+  Proof.
+    rewrite /τR2rP. by rewrite [_ -> _] contra !neg_rsat2.
+  Qed.
+
+  Lemma contra_τR2rTP :
+    τR2rTP <-> (forall P1 P2 S, ((exists C__T t1 t2, sem__T ( plug__T (P1 ↓) C__T) t1 /\
+                                         sem__T ( plug__T (P2 ↓) C__T) t2 /\
+                                       ~ (τ S) (t1, t2)) ->
+                          (exists C__S s1 s2, sem__S (plug__S P1 C__S) s1 /\
+                                        sem__S (plug__S P2 C__S) s2 /\
+                                       ~ S (s1, s2)))).
+  Proof.
+    rewrite /τR2rTP.
+    split => H P1 P2 S; by move/contra_τR2rP: (H P1 P2 S).
+  Qed.
+
+  Theorem G_σR2rTP_iff_τR2rTP :
+    (Galois_fst τ σ) -> (Galois_snd τ σ) -> (σR2rTP <-> τR2rTP).
+  Proof.
+    move => G1 G2. split.
+    - move => Hσ P1 P2 S Hrsat_src. apply: (Hσ P1 P2 (τ S)).
+      apply: rsat2_upper_closed. exact Hrsat_src. by apply: G1.
+    - move => Hτ P1 P2 T Hrrsat_tgt.
+      have H : rsat__T (P1 ↓) (P2 ↓) (τ (σ T)) by apply: Hτ.
+      apply: rsat2_upper_closed. exact H. by apply: G2.
+  Qed.
+
+  Corollary Adj_σR2rTP_iff_τR2rTP :
+    Adjunction_law τ σ -> (σR2rTP <-> τR2rTP).
+  Proof.
+    rewrite Galois_equiv. move => [ms [mt [G1 G2]]].
+      by apply: G_σR2rTP_iff_τR2rTP.
+  Qed.
+
+End Robust2relPreservation.
