RobustSafetyCriterion.v
@@ -1,0 +1,119 @@
+From mathcomp Require Import all_ssreflect.
+
+Set Implicit Arguments.
+Unset Printing Implicit Defensive.
+
+Require Import ClassicalExtras.
+Require Import MyNotation.
+Require Import Setoid.
+Require Import FunctionalExtensionality.
+Require Import Setoid.
+
+Require Import Galois.
+Require Import LanguageModel.
+Require Import TraceModel.
+Require Import Properties.
+Require Import ChainModel.
+Require Import RobustTraceProperty.
+Require Import RobustSafetyPreservation.
+Require Import UcoRobustPreservation.
+
+Require Import PropExtensionality.
+Definition prop_extensionality := propositional_extensionality.
+
+Section RobustSafetyCriterion.
+
+   Variable Source Target: Language.
+  Variable compilation_chain : CompilationChain Source Target.
+
+  Variable T_evs S_evs : Events.
+  Variable T_end S_end : Endstates.
+
+  Local Definition trace__S := @trace S_evs S_end.
+  Local Definition finpref__S := @finpref S_evs S_end.
+  Local Definition trace__T := @trace T_evs T_end.
+  Local Definition finpref__T := @finpref T_evs T_end.
+
+  Local Definition prop__S := prop trace__S.
+  Local Definition Safety__S := @Safety S_evs S_end.
+  Local Definition prop__T := prop trace__T.
+  Local Definition Safety__T := @Safety T_evs T_end.
+
+  Variable Source_Semantics : Semantics Source trace__S.
+  Variable Target_Semantics : Semantics Target trace__T.
+
+  Local Definition sem__S := sem Source_Semantics.
+  Local Definition sem__T := sem Target_Semantics.
+  Local Definition prg__S := prg Source.
+  Local Definition prg__T := prg Target.
+  Local Definition sat__S := sat Source_Semantics.
+  Local Definition sat__T := sat Target_Semantics.
+
+  Local Definition cmp := compile_par Source Target compilation_chain.
+
+  Local Notation "P ↓" := (cmp P) (at level 50).
+ (* CA: don't understand why this does not work
+
+   Local Notation " C [ P ] " := (plug _  P C) (at level 50).
+  *)
+  Local Definition plug__S:= plug Source.
+  Local Definition plug__T := plug Target.
+
+  Variable rel : trace__S -> trace__T -> Prop.
+
+  Local Definition adjunction :=  induced_connection rel.
+
+  Local Definition τ' : prop__S -> prop__T := α adjunction.
+  Local Definition σ' : prop__T -> prop__S := γ adjunction.
+
+  Local Definition rel_adjunction_law : Adjunction_law τ' σ' := adjunction_law adjunction.
+
+  Local Definition Cl_τRP := Cl_τRP compilation_chain
+                                    Source_Semantics Target_Semantics
+                                    τ'.
+
+
+  Local Definition σRP := σRP compilation_chain
+                              Source_Semantics Target_Semantics
+                              σ'.
+
+
+  Definition tilde_RSC :=
+    forall P C__T (t : trace__T) (m : finpref__T),
+      prefix m t ->  sem__T (plug__T (P ↓) C__T) t ->
+      (exists C__S t' s, rel s t' /\ prefix m t' /\ sem__S (plug__S P C__S) s).
+
+  Theorem tilde_RSC_σRSP : tilde_RSC <-> (forall P (π__T : prop__T), Safety__T π__T -> σRP P π__T).
+  Proof.
+    have G2 : Galois_snd τ' σ' by firstorder.
+    split.
+    - move => Htilde P π HSafety. setoid_rewrite contra_σRP.
+      move => [C__T [t [Hsemt Hnot_t]]].
+      destruct (HSafety t Hnot_t) as [m [Hpref_m_t m_witness]].
+      destruct (Htilde P C__T t m) as [C__S [t' [s [Hrel_s_t' [Hpref_m_t' Hsem_s]]]]]; auto.
+      exists C__S, s. split; auto => Hσs.
+      have Ht0 : π t'.
+      { apply: G2; auto. now exists s. }
+        by apply: (m_witness t').
+    - move => H_RSP P C__T t m Hpref_m_t Hsemt.
+      have HSafetyπ : Safety__T (fun t' => ~ prefix m t').
+      { move => t'. rewrite -dne => prefix_m_t'.
+        now exists m. }
+      move : (H_RSP P (fun t' => ~ prefix m t') HSafetyπ).
+      setoid_rewrite contra_σRP => Himp. destruct Himp as [C__S [s [Hsem_s Hσ]]].
+      now exists C__T, t.
+      have : ~ (fun s': trace__S => s' = s) ⊆ (σ' (not ∘ prefix m)) by firstorder.
+      rewrite -rel_adjunction_law not_forall_ex_not. move => [t' Ht'].
+      move/not_imp: Ht' => [Ht' HHt'].
+      exists C__S, t', s. repeat (split; auto).
+      destruct Ht' as [s' [Heq Hs']]. by subst.
+        by apply: NNPP.
+  Qed.
+
+  Theorem tilde_RSC_Cl_τRTP : tilde_RSC <-> (forall P (π__S : prop__S), Cl_τRP P π__S).
+  Proof.
+    setoid_rewrite <- (uco_adjuncts _ _ _ safety_uco rel_adjunction_law).
+    by rewrite tilde_RSC_σRSP -Safety_Cl_prop.
+  Qed.
+
+End RobustSafetyCriterion.
