RobustSafetyPreservation.v
@@ -1,0 +1,84 @@
+From mathcomp Require Import all_ssreflect.
+
+Set Implicit Arguments.
+Unset Printing Implicit Defensive.
+
+Require Import ClassicalExtras.
+Require Import MyNotation.
+Require Import Setoid.
+Require Import FunctionalExtensionality.
+Require Import Setoid.
+
+Require Import Galois.
+Require Import LanguageModel.
+Require Import TraceModel.
+Require Import Properties.
+Require Import ChainModel.
+Require Import RobustTraceProperty.
+Require Import UcoRobustPreservation.
+
+Require Import PropExtensionality.
+Definition prop_extensionality := propositional_extensionality.
+
+Section RobustSafetyPreservation.
+
+  Variable Source Target: Language.
+  Variable compilation_chain : CompilationChain Source Target.
+
+  Variable T_evs S_evs : Events.
+  Variable T_end S_end : Endstates.
+
+  Local Definition trace__S := @trace S_evs S_end.
+  Local Definition finpref__S := @finpref S_evs S_end.
+  Local Definition trace__T := @trace T_evs T_end.
+  Local Definition finpref__T := @finpref T_evs T_end.
+
+  Local Definition prop__S := prop trace__S.
+  Local Definition Safety__S := @Safety S_evs S_end.
+  Local Definition prop__T := prop trace__T.
+  Local Definition Safety__T := @Safety T_evs T_end.
+
+  Variable Source_Semantics : Semantics Source trace__S.
+  Variable Target_Semantics : Semantics Target trace__T.
+
+  Local Definition sem__S := sem Source_Semantics.
+  Local Definition sem__T := sem Target_Semantics.
+  Local Definition prg__S := prg Source.
+  Local Definition prg__T := prg Target.
+  Local Definition sat__S := sat Source_Semantics.
+  Local Definition sat__T := sat Target_Semantics.
+
+  Local Definition cmp := compile_par Source Target compilation_chain.
+
+  Local Notation "P ↓" := (cmp P) (at level 50).
+ (* CA: don't understand why this does not work
+
+   Local Notation " C [ P ] " := (plug _  P C) (at level 50).
+  *)
+  Local Definition plug__S:= plug Source.
+  Local Definition plug__T := plug Target.
+
+  Variable σ : prop__T -> prop__S.
+  Variable τ : prop__S -> prop__T.
+
+  Local Definition σRP := σRP compilation_chain
+                              Source_Semantics Target_Semantics
+                              σ.
+
+  Definition Cl_τRP := τRP compilation_chain
+                           Source_Semantics Target_Semantics
+                           (Cl ∘ τ).
+
+  Theorem σSafetyP_Cl_τTP :
+    (Adjunction_law τ σ) ->
+    ( (forall P (π__T : prop__T), Safety π__T -> σRP P π__T) <->
+      (forall P (π__S : prop__S), Cl_τRP P π__S)).
+  Proof.
+    move => H_adj.
+    setoid_rewrite <- (@uco_adjuncts _ _ _ _ _ _ _ σ τ safety_uco).
+    rewrite -Safety_Cl_prop.
+    reflexivity.
+    assumption.
+  Qed.
+
+End RobustSafetyPreservation.
