SSCHCriterion.v
@@ -1,0 +1,123 @@
+From mathcomp Require Import all_ssreflect.
+
+Set Implicit Arguments.
+Unset Printing Implicit Defensive.
+
+Require Import ClassicalExtras.
+Require Import MyNotation.
+Require Import Setoid.
+Require Import FunctionalExtensionality.
+Require Import Setoid.
+
+Require Import Galois.
+Require Import LanguageModel.
+Require Import TraceModel.
+Require Import Properties.
+Require Import ChainModel.
+Require Import SSCHPreservation.
+Require Import TraceCriterion.
+
+Require Import PropExtensionality.
+Definition prop_extensionality := propositional_extensionality.
+
+Section SSCHCriterion.
+
+  Variable Source Target: Language.
+  Variable compilation_chain : CompilationChain Source Target.
+
+  (*CA: we don't need a particular structure of traces to define preservation
+        e.g. traces = values or our defn of traces both make sense
+   *)
+  Variable trace__S trace__T : Set.
+
+  Local Definition prop__S := prop trace__S.
+  Local Definition prop__T := prop trace__T.
+  Local Definition hprop__S := hprop trace__S.
+  Local Definition hprop__T := hprop trace__T.
+
+
+  Variable Source_Semantics : Semantics Source trace__S.
+  Variable Target_Semantics : Semantics Target trace__T.
+
+  Local Definition sem__S := sem Source_Semantics.
+  Local Definition sem__T := sem Target_Semantics.
+  Local Definition beh__S := beh Source_Semantics.
+  Local Definition beh__T := beh Target_Semantics.
+  Local Definition prg__S := prg Source.
+  Local Definition prg__T := prg Target.
+  Local Definition ctx__S := ctx Source.
+  Local Definition ctx__T := ctx Target.
+  Local Definition hsat__S := hsat Source_Semantics.
+  Local Definition hsat__T := hsat Target_Semantics.
+
+  Local Definition cmp := compile_whole Source Target compilation_chain.
+
+  Local Notation "P ↓" := (cmp P) (at level 50).
+
+  Variable rel : trace__S -> trace__T -> Prop.
+
+  Local Definition adjunction :=  induced_connection rel.
+
+  Local Definition τ' : prop__S -> prop__T := α adjunction.
+  Local Definition σ' : prop__T -> prop__S := γ adjunction.
+
+  Local Definition rel_adjunction_law : Adjunction_law τ' σ' := adjunction_law adjunction.
+
+  Lemma τ_mono : monotone τ'.
+  Proof. move/Galois_equiv: rel_adjunction_law. by move => [H1 H2]. Qed.
+
+  Definition rel_TC : Prop := rel_TC  compilation_chain
+                                   Source_Semantics Target_Semantics
+                                   rel.
+
+  Local Definition sCl_σ : hprop__T -> hprop__S := sCl_σ σ'.
+  Local Definition sCl_τ : hprop__S -> hprop__T := sCl_τ τ'.
+
+  Local Definition sCl_τhP := sCl_τhP compilation_chain
+                                      Source_Semantics Target_Semantics
+                                      τ'.
+
+
+  Local Definition sCl_σhP := sCl_σhP compilation_chain
+                                      Source_Semantics Target_Semantics
+                                      σ'.
+
+
+  Lemma sCl_σhP_sCl_τhP : (forall (W : prg__S) (H__T : hprop__T), SSC H__T ->  sCl_σhP W H__T) <->
+                          (forall (W : prg__S) (H__S : hprop__S), SSC H__S -> sCl_τhP W H__S).
+  Proof.
+    split.
+    + move => Hσ P H__S ssc_H rsat_source.
+      have rsat_sigma_tau : hsat__S P (sCl_σ (sCl_τ H__S)).
+      { apply: hsat_upper_closed. exact rsat_source.
+        apply: Galois_snd_lift. exact rel_adjunction_law. exact ssc_H. }
+      have τ_ssc : SSC (sCl_τ H__S) by apply: sCl_SCH.
+      exact (Hσ P (sCl_τ H__S) τ_ssc rsat_sigma_tau).
+    + move => Hτ P H__T ssc_H rsat_source.
+      have h_ssc: SSC (sCl_σ H__T) by apply: sCl_SCH.
+      move: (Hτ P (sCl_σ H__T) h_ssc rsat_source).
+      move => HHH. eapply hsat_upper_closed. exact HHH.
+      apply: Galois_fst_lift; eauto. exact rel_adjunction_law.
+  Qed.
+
+  Theorem rel_TC_sClτSCHP : rel_TC <-> (forall (P : prg__S) (H__S : hprop__S), SSC H__S -> sCl_τhP P H__S).
+  Proof.
+    setoid_rewrite rel_TC'.
+    split.
+    - move => Htilde P H H_ssc Hsrc.
+      exists (τ' (beh__S P)). split.
+      + rewrite /lift. exists (beh__S P).
+        split; auto. exact: (Htilde P).
+    - move => Hτ W.
+      have Hssc: SSC (fun b: prop__S => b ⊆ beh__S W) by firstorder.
+      have Hfoo: hsat__S W (fun b: prop__S => b ⊆ beh__S W) by rewrite /hsat__S.
+      move: (Hτ W _ Hssc Hfoo).
+      move => [b__T [[b__S [H1 H2]] H3]]. subst.
+      apply: subset_trans.
+      exact H3. by apply: τ_mono.
+  Qed.
+
+  Theorem rel_TC_sCl_σRSCHP : rel_TC <-> (forall (W : prg__S) (H__T : hprop__T), SSC H__T ->  sCl_σhP W H__T).
+  Proof. by rewrite sCl_σhP_sCl_τhP rel_TC_sClτSCHP. Qed.
+
+End SSCHCriterion.
