Stream.v
@@ -1,0 +1,116 @@
+Require Import List.
+
+CoInductive stream {A : Type} :=
+   scons (e : A) (s : stream) : stream.
+
+Fixpoint list_stream_prefix {A : Type} (l : list A) (s : stream) :=
+  match l, s with
+  | nil, _ => True
+  | cons a1 l1, scons a2 s2 => (a1 = a2) /\ (list_stream_prefix l1 s2)
+  end.
+
+Fixpoint list_list_prefix {A : Type} (l1 l2 : list A) :=
+  match l1, l2 with
+  | nil, _ => True
+  | cons a1 l1, cons a2 l2 => (a1 = a2) /\ list_list_prefix l1 l2
+  | _, _ => False
+  end.
+
+Lemma list_list_prefix_ref {A : Type} (l : list A) : list_list_prefix l l.
+Proof. now induction l. Qed.
+
+Lemma list_list_prefix_asym {A : Type} : forall (l1 l2 : list A),
+    list_list_prefix l1 l2 -> list_list_prefix l2 l1 -> l1 = l2.
+Proof.
+  induction l1, l2; try now auto.
+  simpl. intros [afoo Hpref] [afoo' Hpref']; subst; now rewrite (IHl1 l2).
+Qed.
+
+Lemma list_list_prefix_trans {A : Type} : forall l1 l2 l3 : list A,
+  list_list_prefix l1 l2 -> list_list_prefix l2 l3 -> list_list_prefix l1 l3.
+Proof.
+  induction l1; try now auto.
+  intros [] [] H1 H2; inversion H1; inversion H2; subst.
+  simpl. firstorder.
+Qed.
+
+Lemma list_stream_prefix_trans {A : Type} : forall (l1 l2 : list A) (s : stream),
+    list_list_prefix l1 l2 -> list_stream_prefix l2 s ->
+    list_stream_prefix l1 s.
+Proof.
+  induction l1; auto.
+  + intros [] [] Hpref1 Hpref2; inversion Hpref1; inversion Hpref2; subst.
+    simpl. split; auto; now apply (IHl1 l s).
+Qed.
+
+Fixpoint app_list_stream {A : Type} (l : list A) (s : stream) :=
+  match l with
+  | nil => s
+  | e :: l => scons e (app_list_stream l s)
+  end.
+
+Lemma app_list_stream_app {A : Type} (l1 l2 : list A) (s : stream) :
+  app_list_stream (l1 ++ l2) s = app_list_stream l1 (app_list_stream l2 s).
+Proof.
+  induction l1.
+  - eauto.
+  - simpl; now rewrite IHl1.
+Qed.
+
+Lemma list_stream_prefix_app {A : Type} :
+  forall (l' : list A) l s0, list_stream_prefix l s0 -> list_stream_prefix (l' ++ l) (app_list_stream l' s0).
+Proof.
+  intros l'.
+  induction l'.
+  - eauto.
+  - intros l s0 H.
+    simpl. split; eauto using IHl'.
+Qed.
+
+Lemma list_list_prefix_stream_app {A : Type} :
+  forall (l' l : list A) s0, list_list_prefix l' l -> list_stream_prefix l' (app_list_stream l s0).
+Proof.
+  induction l'.
+  - eauto.
+  - destruct l. intros s0 H. inversion H.
+    intros s0 H. simpl in *. destruct H; subst; split; eauto using IHl'.
+Qed.
+
+Lemma list_list_prefix_app {A : Type} : forall (l : list A) l' l'',
+    list_list_prefix l' l'' -> list_list_prefix (l ++ l') (l ++ l'').
+Proof.
+  induction l.
+  eauto.
+  intros l' l'' H. split; eauto.
+Qed.
+
+CoInductive stream_eq {A : Type} : stream -> stream -> Prop :=
+| stream_eq_scons : forall (e : A) s1 s2, stream_eq s1 s2 -> stream_eq (scons e s1) (scons e s2).
+
+Lemma stream_eq_refl : forall {A : Type} (s : @stream A), stream_eq s s.
+Proof.
+  cofix Hfix.
+  intros A s.
+  destruct s.
+  constructor.
+  apply Hfix.
+Qed.
+Hint Resolve stream_eq_refl.
+
+Lemma stream_eq_trans : forall {A : Type} (s1 s2 s3 : @stream A), stream_eq s1 s2 -> stream_eq s2 s3 -> stream_eq s1 s3.
+Proof.
+  cofix Hfix.
+  intros A s1 s2 s3 H H0.
+  destruct s1, s2, s3.
+  inversion H; inversion H0; subst.
+  econstructor.
+  eapply Hfix. eauto. eauto.
+Qed.
+
+Lemma stream_eq_sym : forall {A : Type} (s1 s2 : @stream A), stream_eq s1 s2 -> stream_eq s2 s1.
+Proof.
+  cofix Hfix.
+  intros A s1 s2 H.
+  inversion H; subst.
+  econstructor; eauto.
+Qed.
