TraceCriterion.v
@@ -1,0 +1,176 @@
+From mathcomp Require Import all_ssreflect.
+
+Set Implicit Arguments.
+Unset Printing Implicit Defensive.
+
+Require Import ClassicalExtras.
+Require Import MyNotation.
+Require Import Setoid.
+Require Import FunctionalExtensionality.
+Require Import Setoid.
+
+Require Import Galois.
+Require Import LanguageModel.
+Require Import TraceModel.
+Require Import Properties.
+Require Import ChainModel.
+Require Import Def.
+
+Require Import PropExtensionality.
+Definition prop_extensionality := propositional_extensionality.
+
+Section TracePropertiesCriterion.
+
+  Variable Source Target: Language.
+  Variable compilation_chain : CompilationChain Source Target.
+
+  (*CA: we don't need a particular structure of traces to define preservation
+        e.g. traces = values or our defn of traces both make sense
+   *)
+  Variable trace__S trace__T : Type.
+
+  Local Definition prop__S := prop trace__S.
+  Local Definition prop__T := prop trace__T.
+
+  Variable Source_Semantics : Semantics Source trace__S.
+  Variable Target_Semantics : Semantics Target trace__T.
+
+  Local Definition sem__S := sem Source_Semantics.
+  Local Definition beh__S := beh Source_Semantics.
+  Local Definition sem__T := sem Target_Semantics.
+  Local Definition beh__T := beh Target_Semantics.
+  Local Definition prg__S := prg Source.
+  Local Definition prg__T := prg Target.
+  Local Definition sat__S := sat Source_Semantics.
+  Local Definition sat__T := sat Target_Semantics.
+
+  Local Definition cmp := compile_whole Source Target compilation_chain.
+
+  Local Notation "W ↓" := (cmp W) (at level 50).
+
+  Variable rel : trace__S -> trace__T -> Prop.
+
+  Local Definition adjunction :=  induced_connection rel.
+
+  Local Definition τ' : prop__S -> prop__T := α adjunction.
+  Local Definition σ' : prop__T -> prop__S := γ adjunction.
+
+  Local Definition rel_adjunction_law : Adjunction_law τ' σ' := adjunction_law adjunction.
+
+  Definition rel_TC := forall W t, sem__T (W ↓) t -> exists s, rel s t /\ sem__S W s.
+
+  Lemma rel_TC' : rel_TC <-> (forall W, beh__T (W ↓) ⊆ (τ' (beh__S W))).
+  Proof.
+    rewrite /τ' /α //= /low_rel;
+    split => H W t__T Wcmp_t; specialize (H W t__T Wcmp_t); firstorder.
+  Qed.
+
+
+  Local Definition τTP := τTP compilation_chain
+                          Source_Semantics Target_Semantics
+                          τ'.
+
+
+  Local Definition σTP := σTP compilation_chain
+                              Source_Semantics Target_Semantics
+                              σ'.
+
+
+  Lemma σTP_τTP : σTP <-> τTP.
+  Proof. apply: Adj_σTP_iff_τTP. by apply: rel_adjunction_law. Qed.
+
+
+  Theorem rel_TC_τTP : rel_TC <-> τTP.
+
+  Proof.
+    setoid_rewrite contra_τTP. split.
+    - move => Htilde W π [t [Hsemt Hτ]].
+      destruct (Htilde W t Hsemt) as [s [Hrel_s_t Hsems]].
+      exists s. split; auto. move => s_in_π. apply: Hτ. by exists s.
+    - move => Hτ W t Hsemt. specialize (Hτ W (fun s => ~ rel s t)).
+      case: Hτ.
+      { exists t. split; auto. unfold τ'. move => [s [Hc Hcc]] //=. }
+      move => s [Hsems H]. exists s. split; auto; by apply: NNPP.
+  Qed.
+
+  Theorem rel_TC_σTP : rel_TC <-> σTP.
+  Proof. by rewrite σTP_τTP rel_TC_τTP. Qed.
+
+
+  (* rel version of forward compiler correctness *)
+  Definition rel_FC1 : Prop :=
+    forall W s, sem__S W s -> exists t, rel s t /\ sem__T (W ↓) t.
+
+  Definition σ_fwd : prop__T -> prop__S :=
+    fun π__T : prop__T =>
+      (fun s => exists t, rel s t /\ π__T t).
+  
+  Lemma Galois_fwd_implies_total_rel :
+  Adjunction_law τ' σ_fwd -> (total rel).
+  Proof.
+    move/Galois_equiv => [monotau [monosig [G1 G2]]] s.
+    have Hs: (σ_fwd (τ' (fun s' => s' = s))) s by apply: G1.   
+    destruct Hs as [t Hs]. now exists t.
+  Qed.
+
+  Lemma σ_σ_fwd : σ' = σ_fwd <-> (forall t__S, exists! t__T, rel t__S t__T).
+  Proof.
+    split.
+    + move => H_eq t__S.
+      have adj_fwd: Adjunction_law τ' σ_fwd.
+      { rewrite -H_eq. exact rel_adjunction_law. } 
+      have: exists t__T, rel t__S t__T by apply: Galois_fwd_implies_total_rel.   
+      move => [t__T rel_s_t].
+      exists t__T. split; auto. move => t__T' rel_s_t'.
+      have H: τ' (σ_fwd (eq t__T)) t__T'.
+      { exists t__S. split;auto. by exists t__T. }
+      have G2: Galois_snd τ' σ_fwd. { move/Galois_equiv: adj_fwd. by intuition. }  
+        by apply: (G2 (eq t__T) t__T' H).
+    + move => Htot. apply: functional_extensionality => π__t.
+      apply: functional_extensionality => t__S. 
+      rewrite /σ_fwd /σ' /γ /= /up_rel. 
+      apply: prop_extensionality. split.
+      - by firstorder.
+      - move => [t__T [πt_tT rel_ts_tt]] t__T' H'.
+        destruct (Htot t__S) as [t Ht].
+        have [eq1 eq2] : t = t__T' /\ t = t__T by split; apply Ht.
+        now subst.
+  Qed.
+        
+  Lemma rel_FC1' : rel_FC1 <-> forall W, beh__S W ⊆ σ_fwd (beh__T (W ↓)).
+  Proof.
+    split.
+    - rewrite /σ_fwd => Hrel W s behWs.
+      exact (Hrel W s behWs).
+    - move => Hrel' W s behWs. exact (Hrel' W s behWs).
+  Qed.
+
+  (* another rel version of forward compiler correctness
+     CA: this ensures rel_TC + rel_FC2 -> rel_HC
+   *)
+
+  Definition rel_FC2 : Prop :=
+    forall W s, sem__S W s -> (forall t, rel s t -> sem__T (W ↓) t).
+
+  Lemma rel_FC2' : rel_FC2 <-> (forall W, beh__S W ⊆ σ' (beh__T (W ↓))).
+  Proof. firstorder. Qed.
+
+
+  (* if the Target semantics is deterministic than
+     forward compiler correctness implies target compiler correctness
+  *)
+  Theorem trg_determinism_relFC1_relTC :
+    (forall W__T : prg__T, exists! t__W, sem__T W__T t__W) ->
+    rel_FC1 -> rel_TC.
+  Proof.
+    move => trg_det fcc W t semWt.
+    destruct (trg_det (W ↓)) as [t__w [semWt__W Heq]].
+    destruct (non_empty_sem  Source_Semantics W) as [s semWs].
+    exists s. split; auto.
+    destruct (fcc W s semWs) as [t' [rel_s_t' semWt']].
+    move: (Heq t semWt) (Heq t' semWt'). move => H1 H2.
+      by rewrite -H1 H2.
+  Qed.
+
+End TracePropertiesCriterion.
+
